@prefix : <http://inia.linkeddata.es/def/datasets#> .
@prefix dc: <http://purl.org/dc/elements/1.1/> .
@prefix vs: <http://www.w3.org/2003/06/sw-vocab-status/ns#> .
@prefix geo: <http://www.w3.org/2003/01/geo/wgs84_pos#> .
@prefix owl: <http://www.w3.org/2002/07/owl#> .
@prefix rdf: <http://www.w3.org/1999/02/22-rdf-syntax-ns#> .
@prefix wot: <http://xmlns.com/wot/0.1/> .
@prefix xml: <http://www.w3.org/XML/1998/namespace> .
@prefix xsd: <http://www.w3.org/2001/XMLSchema#> .
@prefix foaf: <http://xmlns.com/foaf/0.1/> .
@prefix prov: <http://www.w3.org/ns/prov#> .
@prefix rdfs: <http://www.w3.org/2000/01/rdf-schema#> .
@prefix vann: <http://purl.org/vocab/vann/> .
@prefix dcterms: <http://purl.org/dc/terms/> .

<https://w3id.org/def/inia#> a owl:Ontology ;
	owl:imports <http://purl.org/spar/datacite/> , <http://www.w3.org/ns/org#> , <http://xmlns.com/foaf/0.1/> ;
	rdfs:comment "Esta ontología representa los datasets publicados por el INIA"@en ;
	dcterms:modified "2017-23-08"^^xsd:date ;
	dc:title "Ontología datasets INIA"@en ;
	vann:preferredNamespacePrefix "inia" ;
	owl:versionInfo "0.0.1" ;
	dcterms:license <http://purl.org/NET/rdflicense/cc-by4.0> ;
	vann:preferredNamespaceUri "https://w3id.org/def/inia#" ;
	dc:publisher <http://www.oeg-upm.net/> .
# 
# 
# #################################################################
# #
# #    Annotation properties
# #
# #################################################################
# 
# 
# http://purl.org/dc/elements/1.1/contributor

dc:contributor a owl:AnnotationProperty .
# 
# http://purl.org/dc/elements/1.1/coverage

dc:coverage a owl:AnnotationProperty .
# 
# http://purl.org/dc/elements/1.1/creator

dc:creator a owl:AnnotationProperty .
# 
# http://purl.org/dc/elements/1.1/format

dc:format a owl:AnnotationProperty .
# 
# http://purl.org/dc/elements/1.1/identifier

dc:identifier a owl:AnnotationProperty .
# 
# http://purl.org/dc/elements/1.1/language

dc:language a owl:AnnotationProperty .
# 
# http://purl.org/dc/elements/1.1/publisher

dc:publisher a owl:AnnotationProperty .
# 
# http://purl.org/dc/elements/1.1/relation

dc:relation a owl:AnnotationProperty .
# 
# http://purl.org/dc/elements/1.1/rights

dc:rights a owl:AnnotationProperty .
# 
# http://purl.org/dc/elements/1.1/source

dc:source a owl:AnnotationProperty .
# 
# http://purl.org/dc/elements/1.1/subject

dc:subject a owl:AnnotationProperty .
# 
# http://purl.org/dc/elements/1.1/type

dc:type a owl:AnnotationProperty .
# 
# http://purl.org/dc/terms/abstract

dcterms:abstract a owl:AnnotationProperty ;
	rdfs:subPropertyOf dc:description .
# 
# http://purl.org/dc/terms/accessRights

dcterms:accessRights a owl:AnnotationProperty ;
	rdfs:subPropertyOf dc:rights ;
	rdfs:range dcterms:RightsStatement .
# 
# http://purl.org/dc/terms/alternative

dcterms:alternative a owl:AnnotationProperty ;
	rdfs:subPropertyOf dc:title ;
	rdfs:range rdfs:Literal .
# 
# http://purl.org/dc/terms/available

dcterms:available a owl:AnnotationProperty ;
	rdfs:subPropertyOf dc:date ;
	rdfs:range rdfs:Literal .
# 
# http://purl.org/dc/terms/bibliographicCitation

dcterms:bibliographicCitation a owl:AnnotationProperty ;
	rdfs:subPropertyOf dc:identifier ;
	rdfs:range rdfs:Literal ;
	rdfs:domain dcterms:BibliographicResource .
# 
# http://purl.org/dc/terms/conformsTo

dcterms:conformsTo a owl:AnnotationProperty ;
	rdfs:subPropertyOf dc:relation ;
	rdfs:range dcterms:Standard .
# 
# http://purl.org/dc/terms/contributor

dcterms:contributor a owl:AnnotationProperty ;
	rdfs:subPropertyOf dc:contributor ;
	rdfs:range dcterms:Agent .
# 
# http://purl.org/dc/terms/coverage

dcterms:coverage a owl:AnnotationProperty ;
	rdfs:subPropertyOf dc:coverage ;
	rdfs:range dcterms:LocationPeriodOrJurisdiction .
# 
# http://purl.org/dc/terms/created

dcterms:created a owl:AnnotationProperty ;
	rdfs:subPropertyOf dc:date ;
	rdfs:range rdfs:Literal .
# 
# http://purl.org/dc/terms/creator

dcterms:creator a owl:AnnotationProperty ;
	rdfs:subPropertyOf dc:creator ;
	rdfs:range dcterms:Agent .
# 
# http://purl.org/dc/terms/date

dcterms:date a owl:AnnotationProperty ;
	rdfs:subPropertyOf dc:date ;
	rdfs:range rdfs:Literal .
# 
# http://purl.org/dc/terms/dateAccepted

dcterms:dateAccepted a owl:AnnotationProperty ;
	rdfs:subPropertyOf dc:date ;
	rdfs:range rdfs:Literal .
# 
# http://purl.org/dc/terms/dateCopyrighted

dcterms:dateCopyrighted a owl:AnnotationProperty ;
	rdfs:subPropertyOf dc:date ;
	rdfs:range rdfs:Literal .
# 
# http://purl.org/dc/terms/dateSubmitted

dcterms:dateSubmitted a owl:AnnotationProperty ;
	rdfs:subPropertyOf dc:date ;
	rdfs:range rdfs:Literal .
# 
# http://purl.org/dc/terms/description

dcterms:description a owl:AnnotationProperty ;
	rdfs:subPropertyOf dc:description .
# 
# http://purl.org/dc/terms/extent

dcterms:extent a owl:AnnotationProperty ;
	rdfs:subPropertyOf dc:format ;
	rdfs:range dcterms:SizeOrDuration .
# 
# http://purl.org/dc/terms/format

dcterms:format a owl:AnnotationProperty ;
	rdfs:subPropertyOf dc:format ;
	rdfs:range dcterms:MediaTypeOrExtent .
# 
# http://purl.org/dc/terms/hasFormat

dcterms:hasFormat a owl:AnnotationProperty ;
	rdfs:subPropertyOf dc:relation .
# 
# http://purl.org/dc/terms/hasPart

dcterms:hasPart a owl:AnnotationProperty ;
	rdfs:subPropertyOf dc:relation .
# 
# http://purl.org/dc/terms/hasVersion

dcterms:hasVersion a owl:AnnotationProperty ;
	rdfs:subPropertyOf dc:relation .
# 
# http://purl.org/dc/terms/identifier

dcterms:identifier a owl:AnnotationProperty ;
	rdfs:subPropertyOf dc:identifier ;
	rdfs:range rdfs:Literal .
# 
# http://purl.org/dc/terms/isFormatOf

dcterms:isFormatOf a owl:AnnotationProperty ;
	rdfs:subPropertyOf dc:relation .
# 
# http://purl.org/dc/terms/isPartOf

dcterms:isPartOf a owl:AnnotationProperty ;
	rdfs:subPropertyOf dc:relation .
# 
# http://purl.org/dc/terms/isReferencedBy

dcterms:isReferencedBy a owl:AnnotationProperty ;
	rdfs:subPropertyOf dc:relation .
# 
# http://purl.org/dc/terms/isReplacedBy

dcterms:isReplacedBy a owl:AnnotationProperty ;
	rdfs:subPropertyOf dc:relation .
# 
# http://purl.org/dc/terms/isRequiredBy

dcterms:isRequiredBy a owl:AnnotationProperty ;
	rdfs:subPropertyOf dc:relation .
# 
# http://purl.org/dc/terms/isVersionOf

dcterms:isVersionOf a owl:AnnotationProperty ;
	rdfs:subPropertyOf dc:relation .
# 
# http://purl.org/dc/terms/issued

dcterms:issued a owl:AnnotationProperty ;
	rdfs:subPropertyOf dc:date ;
	rdfs:range rdfs:Literal .
# 
# http://purl.org/dc/terms/language

dcterms:language a owl:AnnotationProperty ;
	rdfs:subPropertyOf dc:language ;
	rdfs:range dcterms:LinguisticSystem .
# 
# http://purl.org/dc/terms/license

dcterms:license a owl:AnnotationProperty ;
	rdfs:subPropertyOf dc:rights ;
	rdfs:range dcterms:LicenseDocument .
# 
# http://purl.org/dc/terms/medium

dcterms:medium a owl:AnnotationProperty ;
	rdfs:subPropertyOf dc:format ;
	rdfs:range dcterms:PhysicalMedium .
# 
# http://purl.org/dc/terms/modified

dcterms:modified a owl:AnnotationProperty ;
	rdfs:subPropertyOf dc:date ;
	rdfs:range rdfs:Literal .
# 
# http://purl.org/dc/terms/publisher

dcterms:publisher a owl:AnnotationProperty ;
	rdfs:subPropertyOf dc:publisher ;
	rdfs:range dcterms:Agent .
# 
# http://purl.org/dc/terms/references

dcterms:references a owl:AnnotationProperty ;
	rdfs:subPropertyOf dc:relation .
# 
# http://purl.org/dc/terms/relation

dcterms:relation a owl:AnnotationProperty ;
	rdfs:subPropertyOf dc:relation .
# 
# http://purl.org/dc/terms/replaces

dcterms:replaces a owl:AnnotationProperty ;
	rdfs:subPropertyOf dc:relation .
# 
# http://purl.org/dc/terms/requires

dcterms:requires a owl:AnnotationProperty ;
	rdfs:subPropertyOf dc:relation .
# 
# http://purl.org/dc/terms/rights

dcterms:rights a owl:AnnotationProperty ;
	rdfs:subPropertyOf dc:rights ;
	rdfs:range dcterms:RightsStatement .
# 
# http://purl.org/dc/terms/source

dcterms:source a owl:AnnotationProperty ;
	rdfs:subPropertyOf dc:source .
# 
# http://purl.org/dc/terms/spatial

dcterms:spatial a owl:AnnotationProperty ;
	rdfs:subPropertyOf dc:coverage ;
	rdfs:range dcterms:Location .
# 
# http://purl.org/dc/terms/subject

dcterms:subject a owl:AnnotationProperty ;
	rdfs:subPropertyOf dc:subject .
# 
# http://purl.org/dc/terms/tableOfContents

dcterms:tableOfContents a owl:AnnotationProperty ;
	rdfs:subPropertyOf dc:description .
# 
# http://purl.org/dc/terms/temporal

dcterms:temporal a owl:AnnotationProperty ;
	rdfs:subPropertyOf dc:coverage ;
	rdfs:range dcterms:PeriodOfTime .
# 
# http://purl.org/dc/terms/title

dcterms:title a owl:AnnotationProperty ;
	rdfs:subPropertyOf dc:title ;
	rdfs:range rdfs:Literal .
# 
# http://purl.org/dc/terms/type

dcterms:type a owl:AnnotationProperty ;
	rdfs:range rdfs:Class .
# 
# http://purl.org/dc/terms/valid

dcterms:valid a owl:AnnotationProperty ;
	rdfs:subPropertyOf dc:date ;
	rdfs:range rdfs:Literal .
# 
# http://purl.org/vocab/vann/usageNote

vann:usageNote a owl:AnnotationProperty .
# 
# http://www.w3.org/2003/06/sw-vocab-status/ns#term_status

vs:term_status a owl:AnnotationProperty .
# 
# http://www.w3.org/2004/02/skos/core#notation

<http://www.w3.org/2004/02/skos/core#notation> a owl:AnnotationProperty .
# 
# http://www.w3.org/2004/02/skos/core#note

<http://www.w3.org/2004/02/skos/core#note> a owl:AnnotationProperty .
# 
# 
# 
# #################################################################
# #
# #    Datatypes
# #
# #################################################################
# 
# 
# http://def.seegrid.csiro.au/isotc211/iso19150/-2/2012/basic#ISOClassName

<http://def.seegrid.csiro.au/isotc211/iso19150/-2/2012/basic#ISOClassName> a rdfs:Datatype .
# 
# http://purl.org/dc/terms/Box

dcterms:Box a rdfs:Datatype .
# 
# http://purl.org/dc/terms/ISO3166

dcterms:ISO3166 a rdfs:Datatype .
# 
# http://purl.org/dc/terms/ISO639-2

dcterms:ISO639-2 a rdfs:Datatype .
# 
# http://purl.org/dc/terms/ISO639-3

dcterms:ISO639-3 a rdfs:Datatype .
# 
# http://purl.org/dc/terms/Period

dcterms:Period a rdfs:Datatype .
# 
# http://purl.org/dc/terms/Point

dcterms:Point a rdfs:Datatype .
# 
# http://purl.org/dc/terms/RFC1766

dcterms:RFC1766 a rdfs:Datatype .
# 
# http://purl.org/dc/terms/RFC3066

dcterms:RFC3066 a rdfs:Datatype .
# 
# http://purl.org/dc/terms/RFC4646

dcterms:RFC4646 a rdfs:Datatype .
# 
# http://purl.org/dc/terms/RFC5646

dcterms:RFC5646 a rdfs:Datatype .
# 
# http://purl.org/dc/terms/URI

dcterms:URI a rdfs:Datatype .
# 
# http://purl.org/dc/terms/W3CDTF

dcterms:W3CDTF a rdfs:Datatype .
# 
# http://www.w3.org/2001/XMLSchema#date

xsd:date a rdfs:Datatype .
# 
# 
# 
# #################################################################
# #
# #    Object Properties
# #
# #################################################################
# 
# 
# http://dataid.dbpedia.org/ns/core#identifier

<http://dataid.dbpedia.org/ns/core#identifier> a owl:ObjectProperty ;
	rdfs:subPropertyOf <http://purl.org/spar/datacite/hasIdentifier> ;
	a owl:InverseFunctionalProperty ;
	rdfs:range <http://purl.org/spar/datacite/Identifier> ;
	rdfs:comment "A unique identifier for an Agent or Entity (for other, non DataID related identifiers)."@en ;
	rdfs:isDefinedBy <http://dataid.dbpedia.org/ns/core#> ;
	rdfs:label "identifier"@en .
# 
# http://dataid.dbpedia.org/ns/core#latestVersion

<http://dataid.dbpedia.org/ns/core#latestVersion> a owl:ObjectProperty ;
	rdfs:domain prov:Entity ;
	rdfs:range prov:Entity ;
	rdfs:comment "Latest version of a DataId/Dataset/Distribution."@en ;
	rdfs:isDefinedBy <http://dataid.dbpedia.org/ns/core#> ;
	rdfs:label "latest version"@en .
# 
# http://dataid.dbpedia.org/ns/core#nextVersion

<http://dataid.dbpedia.org/ns/core#nextVersion> a owl:ObjectProperty ;
	owl:inverseOf <http://dataid.dbpedia.org/ns/core#previousVersion> ;
	rdfs:comment "Next version of a DataId/Dataset/Distribution."@en ;
	rdfs:isDefinedBy <http://dataid.dbpedia.org/ns/core#> ;
	rdfs:label "next version"@en .
# 
# http://dataid.dbpedia.org/ns/core#openness

<http://dataid.dbpedia.org/ns/core#openness> a owl:ObjectProperty ;
	rdfs:domain <http://dataid.dbpedia.org/ns/core#Dataset> ;
	rdfs:range <http://dataid.dbpedia.org/ns/core#SimpleStatement> ;
	rdfs:comment "General description of how data will be shared. For example embargo periods (if any), outlines of technical mechanisms for dissemination or a definition of whether access will be widely open or restricted to specific groups. In case the Dataset cannot be shared, the reasons for this should be mentioned (e.g. ethical, rules of personal data, intellectual property, commercial, privacy-related, security-related)."@en ;
	rdfs:isDefinedBy <http://dataid.dbpedia.org/ns/dmp#> ;
	rdfs:label "openness"@en .
# 
# http://dataid.dbpedia.org/ns/core#previousVersion

<http://dataid.dbpedia.org/ns/core#previousVersion> a owl:ObjectProperty .
# 
# http://purl.org/dc/elements/1.1/type

dc:type a owl:ObjectProperty .
# 
# http://purl.org/dc/terms/accessRights

dcterms:accessRights a owl:ObjectProperty ;
	rdfs:subPropertyOf dcterms:rights .
# 
# http://purl.org/dc/terms/accrualMethod

dcterms:accrualMethod a owl:ObjectProperty ;
	rdfs:domain <http://purl.org/dc/dcmitype/Collection> ;
	rdfs:range dcterms:MethodOfAccrual .
# 
# http://purl.org/dc/terms/accrualPeriodicity

dcterms:accrualPeriodicity a owl:ObjectProperty ;
	rdfs:domain <http://purl.org/dc/dcmitype/Collection> ;
	rdfs:range dcterms:Frequency .
# 
# http://purl.org/dc/terms/accrualPolicy

dcterms:accrualPolicy a owl:ObjectProperty ;
	rdfs:domain <http://purl.org/dc/dcmitype/Collection> ;
	rdfs:range dcterms:Policy .
# 
# http://purl.org/dc/terms/audience

dcterms:audience a owl:ObjectProperty ;
	rdfs:range dcterms:AgentClass .
# 
# http://purl.org/dc/terms/conformsTo

dcterms:conformsTo a owl:ObjectProperty ;
	rdfs:subPropertyOf dcterms:relation .
# 
# http://purl.org/dc/terms/contributor

dcterms:contributor a owl:ObjectProperty .
# 
# http://purl.org/dc/terms/coverage

dcterms:coverage a owl:ObjectProperty .
# 
# http://purl.org/dc/terms/creator

dcterms:creator a owl:ObjectProperty ;
	rdfs:subPropertyOf dcterms:contributor .
# 
# http://purl.org/dc/terms/educationLevel

dcterms:educationLevel a owl:ObjectProperty ;
	rdfs:subPropertyOf dcterms:audience ;
	rdfs:range dcterms:AgentClass .
# 
# http://purl.org/dc/terms/extent

dcterms:extent a owl:ObjectProperty ;
	rdfs:subPropertyOf dcterms:format .
# 
# http://purl.org/dc/terms/format

dcterms:format a owl:ObjectProperty .
# 
# http://purl.org/dc/terms/hasFormat

dcterms:hasFormat a owl:ObjectProperty ;
	rdfs:subPropertyOf dcterms:relation .
# 
# http://purl.org/dc/terms/hasPart

dcterms:hasPart a owl:ObjectProperty ;
	rdfs:subPropertyOf dcterms:relation .
# 
# http://purl.org/dc/terms/hasVersion

dcterms:hasVersion a owl:ObjectProperty ;
	rdfs:subPropertyOf dcterms:relation .
# 
# http://purl.org/dc/terms/instructionalMethod

dcterms:instructionalMethod a owl:ObjectProperty ;
	rdfs:range dcterms:MethodOfInstruction .
# 
# http://purl.org/dc/terms/isFormatOf

dcterms:isFormatOf a owl:ObjectProperty ;
	rdfs:subPropertyOf dcterms:relation .
# 
# http://purl.org/dc/terms/isPartOf

dcterms:isPartOf a owl:ObjectProperty ;
	rdfs:subPropertyOf dcterms:relation .
# 
# http://purl.org/dc/terms/isReferencedBy

dcterms:isReferencedBy a owl:ObjectProperty ;
	rdfs:subPropertyOf dcterms:relation .
# 
# http://purl.org/dc/terms/isReplacedBy

dcterms:isReplacedBy a owl:ObjectProperty ;
	rdfs:subPropertyOf dcterms:relation .
# 
# http://purl.org/dc/terms/isRequiredBy

dcterms:isRequiredBy a owl:ObjectProperty ;
	rdfs:subPropertyOf dcterms:relation .
# 
# http://purl.org/dc/terms/isVersionOf

dcterms:isVersionOf a owl:ObjectProperty ;
	rdfs:subPropertyOf dcterms:relation .
# 
# http://purl.org/dc/terms/language

dcterms:language a owl:ObjectProperty .
# 
# http://purl.org/dc/terms/license

dcterms:license a owl:ObjectProperty ;
	rdfs:subPropertyOf dcterms:rights .
# 
# http://purl.org/dc/terms/mediator

dcterms:mediator a owl:ObjectProperty ;
	rdfs:subPropertyOf dcterms:audience ;
	rdfs:range dcterms:AgentClass .
# 
# http://purl.org/dc/terms/medium

dcterms:medium a owl:ObjectProperty ;
	rdfs:subPropertyOf dcterms:format ;
	rdfs:domain dcterms:PhysicalResource .
# 
# http://purl.org/dc/terms/provenance

dcterms:provenance a owl:ObjectProperty ;
	rdfs:range dcterms:ProvenanceStatement .
# 
# http://purl.org/dc/terms/publisher

dcterms:publisher a owl:ObjectProperty .
# 
# http://purl.org/dc/terms/references

dcterms:references a owl:ObjectProperty ;
	rdfs:subPropertyOf dcterms:relation .
# 
# http://purl.org/dc/terms/relation

dcterms:relation a owl:ObjectProperty .
# 
# http://purl.org/dc/terms/replaces

dcterms:replaces a owl:ObjectProperty ;
	rdfs:subPropertyOf dcterms:relation .
# 
# http://purl.org/dc/terms/requires

dcterms:requires a owl:ObjectProperty ;
	rdfs:subPropertyOf dcterms:relation .
# 
# http://purl.org/dc/terms/rights

dcterms:rights a owl:ObjectProperty .
# 
# http://purl.org/dc/terms/rightsHolder

dcterms:rightsHolder a owl:ObjectProperty ;
	rdfs:range dcterms:Agent .
# 
# http://purl.org/dc/terms/source

dcterms:source a owl:ObjectProperty ;
	rdfs:subPropertyOf dcterms:relation .
# 
# http://purl.org/dc/terms/spatial

dcterms:spatial a owl:ObjectProperty ;
	rdfs:subPropertyOf dcterms:coverage .
# 
# http://purl.org/dc/terms/temporal

dcterms:temporal a owl:ObjectProperty ;
	rdfs:subPropertyOf dcterms:coverage .
# 
# http://purl.org/dc/terms/type

dcterms:type a owl:ObjectProperty ;
	rdfs:subPropertyOf dc:type .
# 
# http://purl.org/spar/datacite/hasIdentifier

<http://purl.org/spar/datacite/hasIdentifier> a owl:ObjectProperty ;
	rdfs:comment "Relación utilizada entre los recursos o las personas y sus identificadores. Los identificadores se representan mediante instancias de la clase datacite:Identifier pudiendo especializarse en alguna de sus subclases."@es ;
	rdfs:label "tiene identificador"@es .
# 
# http://rdfs.org/ns/void#subset

<http://rdfs.org/ns/void#subset> a owl:ObjectProperty .
# 
# http://rs.tdwg.org/dwc/terms/class

<http://rs.tdwg.org/dwc/terms/class> a owl:ObjectProperty ;
	rdfs:subPropertyOf <https://w3id.org/def/inia#taxonomicalScope> ;
	rdfs:comment "indica la categoría taxonómica clase"@es ;
	rdfs:label "clase"@es , "class"@en .
# 
# http://rs.tdwg.org/dwc/terms/family

<http://rs.tdwg.org/dwc/terms/family> a owl:ObjectProperty ;
	rdfs:subPropertyOf <https://w3id.org/def/inia#taxonomicalScope> ;
	rdfs:comment "indica la categoría taxonómica familia"@es ;
	rdfs:label "familia"@es , "family"@en .
# 
# http://rs.tdwg.org/dwc/terms/genus

<http://rs.tdwg.org/dwc/terms/genus> a owl:ObjectProperty ;
	rdfs:subPropertyOf <https://w3id.org/def/inia#taxonomicalScope> ;
	rdfs:comment "indica la categoría taxonómica género"@es ;
	rdfs:label "genus"@en , "género"@es .
# 
# http://rs.tdwg.org/dwc/terms/kingdom

<http://rs.tdwg.org/dwc/terms/kingdom> a owl:ObjectProperty ;
	rdfs:subPropertyOf <https://w3id.org/def/inia#taxonomicalScope> ;
	rdfs:comment "indica la categoría taxonómica reino"@es ;
	rdfs:label "kingdom"@en , "reino"@es .
# 
# http://rs.tdwg.org/dwc/terms/order

<http://rs.tdwg.org/dwc/terms/order> a owl:ObjectProperty ;
	rdfs:subPropertyOf <https://w3id.org/def/inia#taxonomicalScope> ;
	rdfs:comment "indica la categoría taxonómica orden"@es ;
	rdfs:label "orden"@es , "order"@en .
# 
# http://rs.tdwg.org/dwc/terms/phylum

<http://rs.tdwg.org/dwc/terms/phylum> a owl:ObjectProperty ;
	rdfs:subPropertyOf <https://w3id.org/def/inia#taxonomicalScope> ;
	rdfs:comment "indica la categoría taxonómica filo o división"@es ;
	rdfs:label "filo"@es , "phylum"@en .
# 
# http://rs.tdwg.org/dwc/terms/vernacularName

<http://rs.tdwg.org/dwc/terms/vernacularName> a owl:ObjectProperty ;
	rdfs:comment "Nombre común por ejemplo Melón, algarroba, Pino Carrasco, Cerdo Ibérico."@es ;
	rdfs:label "nombre común"@es .
# 
# http://www.w3.org/ns/dcat#distribution

<http://www.w3.org/ns/dcat#distribution> a owl:ObjectProperty .
# 
# http://www.w3.org/ns/dcat#theme

<http://www.w3.org/ns/dcat#theme> a owl:ObjectProperty ;
	rdfs:domain <http://www.w3.org/ns/dcat#Dataset> ;
	rdfs:range <http://www.w3.org/2004/02/skos/core#Concept> ;
	rdfs:comment "Temática principal del Dataset (en inglés). Se recomienda buscar entre los vocabularios controlados los términos que mas se ajustan a la temática específica del Dataset, en caso de no encontrar la una adecuada, utilizar un termino mas genérico."@es , "The main category of the dataset. A dataset can have multiple themes."@en ;
	rdfs:label "temática"@es , "theme"@en .
# 
# http://xmlns.com/foaf/0.1/isPrimaryTopicOf

foaf:isPrimaryTopicOf a owl:ObjectProperty .
# 
# https://w3id.org/def/inia#cites

<https://w3id.org/def/inia#cites> a owl:ObjectProperty ;
	rdfs:subPropertyOf <https://w3id.org/def/inia#hasRelatedResource> ;
	owl:inverseOf <https://w3id.org/def/inia#isCitedBy> ;
	rdfs:comment "indica que A incluye a B en una cita"@es , "indicates that A includes B in a citation"@en ;
	rdfs:label "cita"@es , "cites"@en ;
	rdfs:seeAlso "https://schema.datacite.org/meta/kernel-4.0/"@es .
# 
# https://w3id.org/def/inia#compiles

<https://w3id.org/def/inia#compiles> a owl:ObjectProperty ;
	rdfs:subPropertyOf <https://w3id.org/def/inia#hasRelatedResource> ;
	owl:inverseOf <https://w3id.org/def/inia#isCompiledBy> ;
	rdfs:comment "Indica que B es el resultado de un evento de compilación o creación utilizando A"@es , "indicates B is the result of a compile or creation event using A"@en ;
	rdfs:label "compila"@es , "compiles"@en ;
	rdfs:seeAlso "https://schema.datacite.org/meta/kernel-4.0/"@es .
# 
# https://w3id.org/def/inia#contactPerson

<https://w3id.org/def/inia#contactPerson> a owl:ObjectProperty ;
	rdfs:subPropertyOf dcterms:contributor ;
	rdfs:label "contact person"@en , "persona de contacto"@es .
# 
# https://w3id.org/def/inia#continues

<https://w3id.org/def/inia#continues> a owl:ObjectProperty ;
	rdfs:subPropertyOf <https://w3id.org/def/inia#hasRelatedResource> ;
	owl:inverseOf <https://w3id.org/def/inia#isContinuedBy> ;
	rdfs:comment "Indica que A es una continuación del trabajo B"@es , "indicates A is a continuation of the work B"@en ;
	rdfs:label "continues"@en , "continúa"@es ;
	rdfs:seeAlso "https://schema.datacite.org/meta/kernel-4.0/"@es .
# 
# https://w3id.org/def/inia#dataCollector

<https://w3id.org/def/inia#dataCollector> a owl:ObjectProperty ;
	rdfs:subPropertyOf dcterms:contributor ;
	rdfs:label "data collector"@en , "recolector de datos"@es .
# 
# https://w3id.org/def/inia#dataCurator

<https://w3id.org/def/inia#dataCurator> a owl:ObjectProperty ;
	rdfs:subPropertyOf dcterms:contributor ;
	rdfs:label "data curator"@en .
# 
# https://w3id.org/def/inia#dataManager

<https://w3id.org/def/inia#dataManager> a owl:ObjectProperty ;
	rdfs:subPropertyOf dcterms:contributor ;
	rdfs:label "data manager"@en , "gestor de datos"@es .
# 
# https://w3id.org/def/inia#developedWithinProject

<https://w3id.org/def/inia#developedWithinProject> a owl:ObjectProperty ;
	rdfs:domain <https://w3id.org/def/inia#Dataset> ;
	rdfs:range foaf:Project ;
	rdfs:comment "proyecto en el cual se ha creado el dataset"@es ;
	rdfs:label "desarrollado en proyecto"@es , "developed within project"@en .
# 
# https://w3id.org/def/inia#distributor

<https://w3id.org/def/inia#distributor> a owl:ObjectProperty ;
	rdfs:subPropertyOf dcterms:contributor ;
	rdfs:label "distribuidor"@es , "distributor"@en .
# 
# https://w3id.org/def/inia#documents

<https://w3id.org/def/inia#documents> a owl:ObjectProperty ;
	rdfs:subPropertyOf <https://w3id.org/def/inia#hasRelatedResource> ;
	owl:inverseOf <https://w3id.org/def/inia#isDocumentedBy> ;
	rdfs:comment "indica que A es documentación sobre B"@es , "indicates A is documentation about B"@en ;
	rdfs:label "documenta"@es , "documents"@en ;
	rdfs:seeAlso "https://schema.datacite.org/meta/kernel-4.0/"@es .
# 
# https://w3id.org/def/inia#editor

<https://w3id.org/def/inia#editor> a owl:ObjectProperty ;
	rdfs:subPropertyOf dcterms:contributor ;
	rdfs:label "editor"@en , "editor"@es .
# 
# https://w3id.org/def/inia#fundedBy

<https://w3id.org/def/inia#fundedBy> a owl:ObjectProperty ;
	rdfs:domain foaf:Project ;
	rdfs:range <http://www.w3.org/ns/org#Organization> ;
	rdfs:comment "relación entre un proyecto y la organización que lo financia"@es ;
	rdfs:label "financiado por"@es , "funded by"@en .
# 
# https://w3id.org/def/inia#hasMetadata

<https://w3id.org/def/inia#hasMetadata> a owl:ObjectProperty ;
	rdfs:subPropertyOf <https://w3id.org/def/inia#hasRelatedResource> ;
	owl:inverseOf <https://w3id.org/def/inia#isMetadataFor> ;
	rdfs:comment "indica que el recurso A tiene como metadatos adicionales el recurso B"@es , "indicates resource A has additional metadata B"@en ;
	rdfs:label "has metadata"@en , "tiene metadatos"@es ;
	rdfs:seeAlso "https://schema.datacite.org/meta/kernel-4.0/"@es .
# 
# https://w3id.org/def/inia#hasPart

<https://w3id.org/def/inia#hasPart> a owl:ObjectProperty ;
	rdfs:subPropertyOf <https://w3id.org/def/inia#hasRelatedResource> ;
	owl:inverseOf <https://w3id.org/def/inia#isPartOf> ;
	rdfs:comment "indica que A incluye a B como una de sus partes"@es , "indicates A includes the part B"@en ;
	rdfs:label "has part"@en , "tiene parte"@es ;
	rdfs:seeAlso "https://schema.datacite.org/meta/kernel-4.0/"@es .
# 
# https://w3id.org/def/inia#hasRelatedResource

<https://w3id.org/def/inia#hasRelatedResource> a owl:ObjectProperty ;
	rdfs:domain <https://w3id.org/def/inia#Resource> ;
	rdfs:range <https://w3id.org/def/inia#Resource> ;
	rdfs:comment "Relación entre dos recursos relacionados entre sí. Esta relación tiene una serie de sub relaciones específicas alineadas con el esquema de data cite."@es ;
	rdfs:label "has related resource"@en , "tiene relación con recurso"@es .
# 
# https://w3id.org/def/inia#hostingInstitution

<https://w3id.org/def/inia#hostingInstitution> a owl:ObjectProperty ;
	rdfs:subPropertyOf dcterms:contributor ;
	rdfs:label "hosting institution"@en , "institución anfitriona"@es .
# 
# https://w3id.org/def/inia#isCitedBy

<https://w3id.org/def/inia#isCitedBy> a owl:ObjectProperty ;
	rdfs:subPropertyOf <https://w3id.org/def/inia#hasRelatedResource> ;
	rdfs:comment "indica que B incluye a A en una cita"@es , "indicates that B includes A in a citation"@en ;
	rdfs:label "es citado por"@es , "is cited by"@en ;
	rdfs:seeAlso "https://schema.datacite.org/meta/kernel-4.0/"@es .
# 
# https://w3id.org/def/inia#isCompiledBy

<https://w3id.org/def/inia#isCompiledBy> a owl:ObjectProperty ;
	rdfs:subPropertyOf <https://w3id.org/def/inia#hasRelatedResource> ;
	rdfs:comment "indica que B es utilizado para compilar o crear A"@es , "indicates B is used to compile or create A"@en ;
	rdfs:label "es compilado por"@es , "is compiled by"@en ;
	rdfs:seeAlso "https://schema.datacite.org/meta/kernel-4.0/"@es .
# 
# https://w3id.org/def/inia#isContinuedBy

<https://w3id.org/def/inia#isContinuedBy> a owl:ObjectProperty ;
	rdfs:subPropertyOf <https://w3id.org/def/inia#hasRelatedResource> ;
	rdfs:comment "indica que A es continuado por el trabajo B"@es , "indicates A is continued by the work B"@en ;
	rdfs:label "es continuado por"@es , "is continued by"@en ;
	rdfs:seeAlso "https://schema.datacite.org/meta/kernel-4.0/"@es .
# 
# https://w3id.org/def/inia#isDerivedFrom

<https://w3id.org/def/inia#isDerivedFrom> a owl:ObjectProperty ;
	rdfs:subPropertyOf <https://w3id.org/def/inia#hasRelatedResource> ;
	owl:inverseOf <https://w3id.org/def/inia#isSourceOf> ;
	rdfs:comment "indica que B es una fuente en la que está basado A"@es , "indicates B is a source upon which A is based"@en ;
	rdfs:label "es derivado de"@es , "is derived from"@en ;
	rdfs:seeAlso "https://schema.datacite.org/meta/kernel-4.0/"@es .
# 
# https://w3id.org/def/inia#isDocumentedBy

<https://w3id.org/def/inia#isDocumentedBy> a owl:ObjectProperty ;
	rdfs:subPropertyOf <https://w3id.org/def/inia#hasRelatedResource> ;
	rdfs:comment "indica que B es la documentación sobre A"@es , "indicates B is documentation about explaining A"@en ;
	rdfs:label "está documentado por"@es , "is documented by"@en ;
	rdfs:seeAlso "https://schema.datacite.org/meta/kernel-4.0/"@es .
# 
# https://w3id.org/def/inia#isIdenticalTo

<https://w3id.org/def/inia#isIdenticalTo> a owl:ObjectProperty ;
	rdfs:subPropertyOf <https://w3id.org/def/inia#hasRelatedResource> ;
	rdfs:comment "Esta relación no debe utilizarse, owl:sameAs debe ser utilizado en su lugar. Se crea sólo para mantener un registro de su existencia en el esquema de datacite."@es , "This relation is not to be used, owl:sameAs should be used instead. It is created just to keep record of its existance in datacite schema."@en , "indicates that A is identical to B, for use when there is a need to register two separate instances of the same resource"@en ;
	rdfs:label "es idéntico a"@es , "isIdenticalTo"@en ;
	rdfs:seeAlso "https://schema.datacite.org/meta/kernel-4.0/"@es ;
	owl:deprecated "true"^^xsd:boolean ;
	vs:term_status "unestable"@es .
# 
# https://w3id.org/def/inia#isMetadataFor

<https://w3id.org/def/inia#isMetadataFor> a owl:ObjectProperty ;
	rdfs:subPropertyOf <https://w3id.org/def/inia#hasRelatedResource> ;
	rdfs:comment "indica que A contiene metadatos adicionales sobre el recurso B"@es , "indicates additional metadata A for a resource B"@en ;
	rdfs:label "es metadatos de"@es , "is metadata for"@en ;
	rdfs:seeAlso "https://schema.datacite.org/meta/kernel-4.0/"@es .
# 
# https://w3id.org/def/inia#isNewVersionOf

<https://w3id.org/def/inia#isNewVersionOf> a owl:ObjectProperty ;
	rdfs:subPropertyOf <http://dataid.dbpedia.org/ns/core#previousVersion> , <https://w3id.org/def/inia#hasRelatedResource> ;
	owl:inverseOf <https://w3id.org/def/inia#isPreviousVersionOf> ;
	rdfs:comment "indica que A es una nueva edición de B, donde la nueva edición ha sido modifcada o actualizada"@es , "indicates A is a new edition of B, where the new edition has been modified or updated"@en ;
	rdfs:label "es nueva versión de"@es , "is new version of"@en ;
	rdfs:seeAlso "https://schema.datacite.org/meta/kernel-4.0/"@es .
# 
# https://w3id.org/def/inia#isOriginalFormOf

<https://w3id.org/def/inia#isOriginalFormOf> a owl:ObjectProperty ;
	rdfs:subPropertyOf <https://w3id.org/def/inia#hasRelatedResource> ;
	owl:inverseOf <https://w3id.org/def/inia#isVariantFormOf> ;
	rdfs:comment "indica que A es la forma origen de B"@es , "indicates A is the original form of B"@en ;
	rdfs:label "es forma original de"@es , "is original form of"@en ;
	rdfs:seeAlso "https://schema.datacite.org/meta/kernel-4.0/"@es .
# 
# https://w3id.org/def/inia#isPartOf

<https://w3id.org/def/inia#isPartOf> a owl:ObjectProperty ;
	rdfs:subPropertyOf dcterms:isPartOf , <https://w3id.org/def/inia#hasRelatedResource> ;
	rdfs:comment "indica que A es una porciónde B, esta relación puede ser utilizada para elementos de una serie"@es , "indicates A is a portion of B; may be used for elements of a series"@en ;
	rdfs:label "es parte de"@es , "is part of"@en ;
	rdfs:seeAlso "https://schema.datacite.org/meta/kernel-4.0/"@es .
# 
# https://w3id.org/def/inia#isPreviousVersionOf

<https://w3id.org/def/inia#isPreviousVersionOf> a owl:ObjectProperty ;
	rdfs:subPropertyOf <http://dataid.dbpedia.org/ns/core#nextVersion> , <https://w3id.org/def/inia#hasRelatedResource> ;
	rdfs:comment "indica que A es una edición previa de B"@es , "indicates A is a previous edition of B"@en ;
	rdfs:label "es versión previa de"@es , "is previous version of"@en ;
	rdfs:seeAlso "https://schema.datacite.org/meta/kernel-4.0/"@es .
# 
# https://w3id.org/def/inia#isReferencedBy

<https://w3id.org/def/inia#isReferencedBy> a owl:ObjectProperty ;
	rdfs:subPropertyOf <https://w3id.org/def/inia#hasRelatedResource> ;
	owl:inverseOf <https://w3id.org/def/inia#references> ;
	rdfs:comment "indica que A es utilizado como fuente de información por B"@es , "indicates A is used as a source of information by B"@en ;
	rdfs:label "es referenciado por"@es , "is referenced by"@en ;
	rdfs:seeAlso "https://schema.datacite.org/meta/kernel-4.0/"@es .
# 
# https://w3id.org/def/inia#isReviewedBy

<https://w3id.org/def/inia#isReviewedBy> a owl:ObjectProperty ;
	rdfs:subPropertyOf <https://w3id.org/def/inia#hasRelatedResource> ;
	owl:inverseOf <https://w3id.org/def/inia#reviews> ;
	rdfs:comment "indica que A es revisado por B"@es , "indicates that A is reviewed by B"@en ;
	rdfs:label "es revisado por"@es , "is reviewed by"@en ;
	rdfs:seeAlso "https://schema.datacite.org/meta/kernel-4.0/"@es .
# 
# https://w3id.org/def/inia#isSourceOf

<https://w3id.org/def/inia#isSourceOf> a owl:ObjectProperty ;
	rdfs:subPropertyOf <https://w3id.org/def/inia#hasRelatedResource> ;
	rdfs:comment "indica que A es una fuente sobre la que B está basado"@es , "indicates A is a source upon which B is based"@en ;
	rdfs:label "es fuente de"@es , "is source of"@en ;
	rdfs:seeAlso "https://schema.datacite.org/meta/kernel-4.0/"@es .
# 
# https://w3id.org/def/inia#isSupplementTo

<https://w3id.org/def/inia#isSupplementTo> a owl:ObjectProperty ;
	rdfs:subPropertyOf <https://w3id.org/def/inia#hasRelatedResource> ;
	owl:inverseOf <https://w3id.org/def/inia#isSupplementedBy> ;
	rdfs:comment "indica que A es un suplemento de B"@es , "indicates that A is a supplement to B"@en ;
	rdfs:label "es suplemento de"@es , "is supplement to"@en ;
	rdfs:seeAlso "https://schema.datacite.org/meta/kernel-4.0/"@es .
# 
# https://w3id.org/def/inia#isSupplementedBy

<https://w3id.org/def/inia#isSupplementedBy> a owl:ObjectProperty ;
	rdfs:subPropertyOf <https://w3id.org/def/inia#hasRelatedResource> ;
	rdfs:comment "indica que B es un suplemento de A"@es , "indicates that B is a supplement to A"@en ;
	rdfs:label "is supplemented by"@en , "se suplementa con"@es ;
	rdfs:seeAlso "https://schema.datacite.org/meta/kernel-4.0/"@es .
# 
# https://w3id.org/def/inia#isVariantFormOf

<https://w3id.org/def/inia#isVariantFormOf> a owl:ObjectProperty ;
	rdfs:subPropertyOf <https://w3id.org/def/inia#hasRelatedResource> ;
	rdfs:comment "indica que A es un variante o forma diferente de B, or ejemplo una forma calculada o calibrada"@es , "indicates A is a variant or different form of B, e.g. calculated or calibrated form or different packaging"@en ;
	rdfs:label "es una variante de"@es , "is variant form of"@en ;
	rdfs:seeAlso "https://schema.datacite.org/meta/kernel-4.0/"@es .
# 
# https://w3id.org/def/inia#producer

<https://w3id.org/def/inia#producer> a owl:ObjectProperty ;
	rdfs:subPropertyOf dcterms:contributor ;
	rdfs:label "producer"@en , "productor"@es .
# 
# https://w3id.org/def/inia#projectLeader

<https://w3id.org/def/inia#projectLeader> a owl:ObjectProperty ;
	rdfs:subPropertyOf dcterms:contributor ;
	rdfs:label "líder de proyecto"@es , "project leader"@en .
# 
# https://w3id.org/def/inia#projectManager

<https://w3id.org/def/inia#projectManager> a owl:ObjectProperty ;
	rdfs:subPropertyOf dcterms:contributor ;
	rdfs:label "jefe de proyecto"@es , "project manager"@en .
# 
# https://w3id.org/def/inia#references

<https://w3id.org/def/inia#references> a owl:ObjectProperty ;
	rdfs:subPropertyOf <https://w3id.org/def/inia#hasRelatedResource> ;
	rdfs:comment "indica que B es utilizado como fuente de información de A"@es , "indicates B is used as a source of information for A"@en ;
	rdfs:label "references"@en , "referencia"@es ;
	rdfs:seeAlso "https://schema.datacite.org/meta/kernel-4.0/"@es .
# 
# https://w3id.org/def/inia#registrationAgency

<https://w3id.org/def/inia#registrationAgency> a owl:ObjectProperty ;
	rdfs:subPropertyOf dcterms:contributor ;
	rdfs:label "agencia de registro"@es , "registration agency"@en .
# 
# https://w3id.org/def/inia#registrationAuthority

<https://w3id.org/def/inia#registrationAuthority> a owl:ObjectProperty ;
	rdfs:subPropertyOf dcterms:contributor ;
	rdfs:label "autoridad de registro"@es , "registration authority"@en .
# 
# https://w3id.org/def/inia#relatedPerson

<https://w3id.org/def/inia#relatedPerson> a owl:ObjectProperty ;
	rdfs:subPropertyOf dcterms:contributor ;
	rdfs:label "persona relacionada"@es , "related person"@en .
# 
# https://w3id.org/def/inia#researchGroup

<https://w3id.org/def/inia#researchGroup> a owl:ObjectProperty ;
	rdfs:subPropertyOf dcterms:contributor ;
	rdfs:label "grupo de investigación"@es , "research group"@en .
# 
# https://w3id.org/def/inia#researcher

<https://w3id.org/def/inia#researcher> a owl:ObjectProperty ;
	rdfs:subPropertyOf dcterms:contributor ;
	rdfs:label "investigador"@es , "researcher"@en .
# 
# https://w3id.org/def/inia#reviews

<https://w3id.org/def/inia#reviews> a owl:ObjectProperty ;
	rdfs:subPropertyOf <https://w3id.org/def/inia#hasRelatedResource> ;
	rdfs:comment "indica que A  es una revisión de B"@es , "indicates that A is a review of B"@en ;
	rdfs:label "reviews"@en , "revisa"@es ;
	rdfs:seeAlso "https://schema.datacite.org/meta/kernel-4.0/"@es .
# 
# https://w3id.org/def/inia#rightsHolder

<https://w3id.org/def/inia#rightsHolder> a owl:ObjectProperty ;
	rdfs:subPropertyOf dcterms:contributor , dcterms:rightsHolder ;
	rdfs:label "rights holder"@en , "titular de derechos"@es .
# 
# https://w3id.org/def/inia#specie

<https://w3id.org/def/inia#specie> a owl:ObjectProperty ;
	rdfs:subPropertyOf <https://w3id.org/def/inia#taxonomicalScope> ;
	rdfs:comment "indica la categoría taxonómica especie"@es ;
	rdfs:label "especie"@es , "specie"@en .
# 
# https://w3id.org/def/inia#sponsor

<https://w3id.org/def/inia#sponsor> a owl:ObjectProperty ;
	rdfs:subPropertyOf dcterms:contributor ;
	rdfs:label "financiador"@es , "sponsor"@en .
# 
# https://w3id.org/def/inia#supervisor

<https://w3id.org/def/inia#supervisor> a owl:ObjectProperty ;
	rdfs:subPropertyOf dcterms:contributor ;
	rdfs:label "supervisor"@en , "supervisor"@es .
# 
# https://w3id.org/def/inia#taxonomicalScope

<https://w3id.org/def/inia#taxonomicalScope> a owl:ObjectProperty ;
	rdfs:comment "Relación genera para indicar el ámbito taxonómico que puede ser especializada por una o mas de sus subpropiedades."@es ;
	rdfs:label "taxonomical scope"@en , "ámbito taxonómico"@es .
# 
# https://w3id.org/def/inia#workPackageLeader

<https://w3id.org/def/inia#workPackageLeader> a owl:ObjectProperty ;
	rdfs:subPropertyOf dcterms:contributor ;
	rdfs:label "líder de paquete de trabajo"@es , "work package leader"@en .
# 
# 
# 
# #################################################################
# #
# #    Data properties
# #
# #################################################################
# 
# 
# http://def.seegrid.csiro.au/isotc211/iso19115/2003/extent#eastBoundLongitude

<http://def.seegrid.csiro.au/isotc211/iso19115/2003/extent#eastBoundLongitude> a owl:DatatypeProperty ;
	rdfs:domain <http://def.seegrid.csiro.au/isotc211/iso19115/2003/extent#GeographicBoundingBox> ;
	rdfs:range xsd:decimal ;
	rdfs:isDefinedBy <http://def.seegrid.csiro.au/isotc211/iso19115/2003/extent> ;
	rdfs:label "east bound longitude"^^xsd:string .
# 
# http://def.seegrid.csiro.au/isotc211/iso19115/2003/extent#northBoundLatitude

<http://def.seegrid.csiro.au/isotc211/iso19115/2003/extent#northBoundLatitude> a owl:DatatypeProperty ;
	rdfs:domain <http://def.seegrid.csiro.au/isotc211/iso19115/2003/extent#GeographicBoundingBox> ;
	rdfs:range xsd:decimal ;
	rdfs:isDefinedBy <http://def.seegrid.csiro.au/isotc211/iso19115/2003/extent> ;
	rdfs:label "north bound latitude"^^xsd:string .
# 
# http://def.seegrid.csiro.au/isotc211/iso19115/2003/extent#southBoundLatitude

<http://def.seegrid.csiro.au/isotc211/iso19115/2003/extent#southBoundLatitude> a owl:DatatypeProperty ;
	rdfs:domain <http://def.seegrid.csiro.au/isotc211/iso19115/2003/extent#GeographicBoundingBox> ;
	rdfs:range xsd:decimal ;
	rdfs:isDefinedBy <http://def.seegrid.csiro.au/isotc211/iso19115/2003/extent> ;
	rdfs:label "south bound latitude"^^xsd:string .
# 
# http://def.seegrid.csiro.au/isotc211/iso19115/2003/extent#westBoundLongitude

<http://def.seegrid.csiro.au/isotc211/iso19115/2003/extent#westBoundLongitude> a owl:DatatypeProperty ;
	rdfs:domain <http://def.seegrid.csiro.au/isotc211/iso19115/2003/extent#GeographicBoundingBox> ;
	rdfs:range xsd:decimal ;
	rdfs:isDefinedBy <http://def.seegrid.csiro.au/isotc211/iso19115/2003/extent> ;
	rdfs:label "west bound longitude"^^xsd:string .
# 
# http://purl.org/dc/terms/abstract

dcterms:abstract a owl:DatatypeProperty ;
	rdfs:subPropertyOf dcterms:description .
# 
# http://purl.org/dc/terms/alternative

dcterms:alternative a owl:DatatypeProperty ;
	rdfs:subPropertyOf dcterms:title .
# 
# http://purl.org/dc/terms/available

dcterms:available a owl:DatatypeProperty ;
	rdfs:subPropertyOf dcterms:date .
# 
# http://purl.org/dc/terms/bibliographicCitation

dcterms:bibliographicCitation a owl:DatatypeProperty ;
	rdfs:subPropertyOf dcterms:identifier .
# 
# http://purl.org/dc/terms/created

dcterms:created a owl:DatatypeProperty ;
	rdfs:subPropertyOf dcterms:date .
# 
# http://purl.org/dc/terms/date

dcterms:date a owl:DatatypeProperty .
# 
# http://purl.org/dc/terms/dateAccepted

dcterms:dateAccepted a owl:DatatypeProperty ;
	rdfs:subPropertyOf dcterms:date .
# 
# http://purl.org/dc/terms/dateCopyrighted

dcterms:dateCopyrighted a owl:DatatypeProperty ;
	rdfs:subPropertyOf dcterms:date .
# 
# http://purl.org/dc/terms/dateSubmitted

dcterms:dateSubmitted a owl:DatatypeProperty ;
	rdfs:subPropertyOf dcterms:date .
# 
# http://purl.org/dc/terms/description

dcterms:description a owl:DatatypeProperty .
# 
# http://purl.org/dc/terms/identifier

dcterms:identifier a owl:DatatypeProperty .
# 
# http://purl.org/dc/terms/issued

dcterms:issued a owl:DatatypeProperty ;
	rdfs:subPropertyOf dcterms:date .
# 
# http://purl.org/dc/terms/modified

dcterms:modified a owl:DatatypeProperty ;
	rdfs:subPropertyOf dcterms:date .
# 
# http://purl.org/dc/terms/tableOfContents

dcterms:tableOfContents a owl:DatatypeProperty ;
	rdfs:subPropertyOf dcterms:description .
# 
# http://purl.org/dc/terms/title

dcterms:title a owl:DatatypeProperty .
# 
# http://purl.org/dc/terms/valid

dcterms:valid a owl:DatatypeProperty ;
	rdfs:subPropertyOf dcterms:date .
# 
# http://www.w3.org/ns/dcat#keyword

<http://www.w3.org/ns/dcat#keyword> a owl:DatatypeProperty ;
	rdfs:domain <http://www.w3.org/ns/dcat#Dataset> ;
	rdfs:range rdfs:Literal ;
	rdfs:comment "A keyword or tag describing the dataset."@en , "Palabra clave asociada al dataset."@es ;
	rdfs:label "keyword"@en , "palabra clave"@es .
# 
# https://w3id.org/def/inia#elementsNumber

<https://w3id.org/def/inia#elementsNumber> a owl:DatatypeProperty ;
	rdfs:domain <https://w3id.org/def/inia#Dataset> ;
	rdfs:comment "Número de instancias de la colección."@es ;
	rdfs:label "elements number"@en , "número de elementos"@es .
# 
# https://w3id.org/def/inia#embargoDate

<https://w3id.org/def/inia#embargoDate> a owl:DatatypeProperty ;
	rdfs:domain <https://w3id.org/def/inia#Dataset> ;
	rdfs:range xsd:date ;
	rdfs:comment "Fecha en la cual se cumple el embargo y pasa a ser un recurso de uso libre."@es ;
	rdfs:label "embargo date"@en , "fecha de embargo"@es .
# 
# https://w3id.org/def/inia#equipment

<https://w3id.org/def/inia#equipment> a owl:DatatypeProperty ;
	rdfs:domain <https://w3id.org/def/inia#Dataset> ;
	rdfs:range xsd:string ;
	rdfs:comment "En caso de ser relevante el instrumento de medida utilizado, marca modelo precisión etc."@es , "Instrumentación de medida"@es ;
	rdfs:label "equipment"@en .
# 
# https://w3id.org/def/inia#finalDate

<https://w3id.org/def/inia#finalDate> a owl:DatatypeProperty ;
	rdfs:subPropertyOf owl:topDataProperty ;
	rdfs:range xsd:date ;
	rdfs:label "Fecha final, relacionada con el ámbito del Dataset. Este atributo suele utilizarse en combinación con inia:startingDate como alternativa a dcterms:temporal."@es , "fecha final"@es , "final date"@en .
# 
# https://w3id.org/def/inia#projectCode

<https://w3id.org/def/inia#projectCode> a owl:DatatypeProperty ;
	rdfs:domain foaf:Project ;
	rdfs:range xsd:string ;
	rdfs:comment "código del proyecto en el que se ha desarrollado un dataset"@es ;
	rdfs:label "código de proyecto"@es , "project code"@en .
# 
# https://w3id.org/def/inia#software

<https://w3id.org/def/inia#software> a owl:DatatypeProperty ;
	rdfs:subPropertyOf owl:topDataProperty ;
	rdfs:domain <https://w3id.org/def/inia#Dataset> ;
	rdfs:range xsd:string ;
	rdfs:comment "Hace referencia al software utilizado para la eleboración del dataset o para su visualización o explotación, nombre, versión, marca."@es ;
	rdfs:label "software"@en , "software"@es .
# 
# https://w3id.org/def/inia#spatialScope

<https://w3id.org/def/inia#spatialScope> a owl:DatatypeProperty ;
	rdfs:range xsd:string ;
	rdfs:comment "Descripción textual del ámbito geográfico relacionado con el contenido o la toma de muestras del Dataset, este metadato está especialmente indicado en los ámbitos de investigación donde es habitual  expresar determinadas zonas de manera textual, península ibérica, cuenca alta del Júcar, sierra de Cazorla, Madrid."@es ;
	rdfs:label "ambito geográfico"@es , "spatial scope"@en .
# 
# https://w3id.org/def/inia#startingDate

<https://w3id.org/def/inia#startingDate> a owl:DatatypeProperty ;
	rdfs:range xsd:date ;
	rdfs:comment "Fecha inicial, relacionada con el ámbito del Dataset ejemplo: fecha inicial de las toma de muestras del material incluido en el Dataset 25/06/1938. Este atributo suele utilizarse en combinación con inia:finalDate como alternativa a dcterms:temporal."@es , "fecha inicial"@es ;
	rdfs:label "starting date"@en .
# 
# https://w3id.org/def/inia#temporalScope

<https://w3id.org/def/inia#temporalScope> a owl:DatatypeProperty ;
	rdfs:range xsd:string ;
	rdfs:comment "Descripción textual periodo de tiempo relacionado con el contenido o la toma de muestras del Dataset, este metadato está especialmente indicado en los ámbitos de investigación donde es habitual  expresar los periodos se de manera textual por ejemplos: siglo XVI, Cretácico, Edad media."@es ;
	rdfs:label "temporal scope"@en , "ámbito temporal"@es .
# 
# 
# 
# #################################################################
# #
# #    Classes
# #
# #################################################################
# 
# 
# http://dataid.dbpedia.org/ns/core#DataId

<http://dataid.dbpedia.org/ns/core#DataId> a owl:Class .
# 
# http://dataid.dbpedia.org/ns/core#Dataset

<http://dataid.dbpedia.org/ns/core#Dataset> a owl:Class ;
	rdfs:subClassOf <http://rdfs.org/ns/void#Dataset> , <http://www.w3.org/ns/dcat#Dataset> , prov:Entity , _:genid1 .

_:genid1 a owl:Restriction ;
	owl:onProperty <http://dataid.dbpedia.org/ns/core#latestVersion> ;
	owl:allValuesFrom <http://dataid.dbpedia.org/ns/core#Dataset> .

<http://dataid.dbpedia.org/ns/core#Dataset> rdfs:subClassOf _:genid2 .

_:genid2 a owl:Restriction ;
	owl:onProperty <http://dataid.dbpedia.org/ns/core#nextVersion> ;
	owl:allValuesFrom <http://dataid.dbpedia.org/ns/core#Dataset> .

<http://dataid.dbpedia.org/ns/core#Dataset> rdfs:subClassOf _:genid3 .

_:genid3 a owl:Restriction ;
	owl:onProperty <http://dataid.dbpedia.org/ns/core#previousVersion> ;
	owl:allValuesFrom <http://dataid.dbpedia.org/ns/core#Dataset> .

<http://dataid.dbpedia.org/ns/core#Dataset> rdfs:subClassOf _:genid4 .

_:genid4 a owl:Restriction ;
	owl:onProperty dcterms:isPartOf ;
	owl:allValuesFrom <http://dataid.dbpedia.org/ns/core#Dataset> .

<http://dataid.dbpedia.org/ns/core#Dataset> rdfs:subClassOf _:genid5 .

_:genid5 a owl:Restriction ;
	owl:onProperty dcterms:language ;
	owl:allValuesFrom <http://lexvo.org/ontology#Language> .

<http://dataid.dbpedia.org/ns/core#Dataset> rdfs:subClassOf _:genid6 .

_:genid6 a owl:Restriction ;
	owl:onProperty dcterms:license ;
	owl:allValuesFrom <http://www.w3.org/ns/odrl/2/Policy> .

<http://dataid.dbpedia.org/ns/core#Dataset> rdfs:subClassOf _:genid7 .

_:genid7 a owl:Restriction ;
	owl:onProperty dcterms:rights ;
	owl:allValuesFrom <http://dataid.dbpedia.org/ns/core#SimpleStatement> .

<http://dataid.dbpedia.org/ns/core#Dataset> rdfs:subClassOf _:genid8 .

_:genid8 a owl:Restriction ;
	owl:onProperty dcterms:spatial ;
	owl:allValuesFrom <http://www.geonames.org/ontology#Feature> .

<http://dataid.dbpedia.org/ns/core#Dataset> rdfs:subClassOf _:genid9 .

_:genid9 a owl:Restriction ;
	owl:onProperty dcterms:temporal ;
	owl:allValuesFrom <http://www.w3.org/2006/time#Interval> .

<http://dataid.dbpedia.org/ns/core#Dataset> rdfs:subClassOf _:genid10 .

_:genid10 a owl:Restriction ;
	owl:onProperty <http://rdfs.org/ns/void#subset> ;
	owl:allValuesFrom <http://dataid.dbpedia.org/ns/core#Dataset> .

<http://dataid.dbpedia.org/ns/core#Dataset> rdfs:subClassOf _:genid11 .

_:genid11 a owl:Restriction ;
	owl:onProperty <http://www.w3.org/ns/dcat#distribution> ;
	owl:allValuesFrom <http://dataid.dbpedia.org/ns/core#Distribution> .

<http://dataid.dbpedia.org/ns/core#Dataset> rdfs:subClassOf _:genid12 .

_:genid12 a owl:Restriction ;
	owl:onProperty foaf:isPrimaryTopicOf ;
	owl:allValuesFrom <http://dataid.dbpedia.org/ns/core#DataId> .

<http://dataid.dbpedia.org/ns/core#Dataset> rdfs:comment """A collection of data, available for access in one or more formats. 
    Dataset resources describe the concept of the dataset, not its manifestation (the data itself), which can be acquired 
    as a Distribution. Datasets are prov:Entities and can be generated by prov:Activities."""@en ;
	rdfs:isDefinedBy <http://dataid.dbpedia.org/ns/core#> ;
	rdfs:label "Dataset"@en .
# 
# http://dataid.dbpedia.org/ns/core#Distribution

<http://dataid.dbpedia.org/ns/core#Distribution> a owl:Class .
# 
# http://dataid.dbpedia.org/ns/core#SimpleStatement

<http://dataid.dbpedia.org/ns/core#SimpleStatement> a owl:Class .
# 
# http://dataid.dbpedia.org/ns/core#Superset

<http://dataid.dbpedia.org/ns/core#Superset> a owl:Class ;
	rdfs:subClassOf <http://dataid.dbpedia.org/ns/core#Dataset> , _:genid13 .

_:genid13 a owl:Restriction ;
	owl:onProperty <http://www.w3.org/ns/dcat#distribution> ;
	owl:maxCardinality "0"^^xsd:nonNegativeInteger .

<http://dataid.dbpedia.org/ns/core#Superset> rdfs:comment """This dedicated version of a dataid:Dataset has exacly one purpose: to point out all its Sub-Datsets with void:subset. 
    A dataid:Superset has no data itself and is therefore prohibited to point out Distributions with dcat:distribution. 
    It can be used in a dataset hierarchy (e.g. as a root dataset), or as a container for other datasets."""@en ;
	rdfs:isDefinedBy <http://dataid.dbpedia.org/ns/core#> ;
	rdfs:label "Superset"@en .
# 
# http://def.seegrid.csiro.au/isotc211/iso19115/2003/extent#GeographicBoundingBox

<http://def.seegrid.csiro.au/isotc211/iso19115/2003/extent#GeographicBoundingBox> a owl:Class ;
	rdfs:subClassOf <http://def.seegrid.csiro.au/isotc211/iso19115/2003/extent#GeographicExtent> , _:genid14 .

_:genid14 a owl:Restriction ;
	owl:onProperty <http://def.seegrid.csiro.au/isotc211/iso19115/2003/extent#eastBoundLongitude> ;
	owl:cardinality "1"^^xsd:nonNegativeInteger .

<http://def.seegrid.csiro.au/isotc211/iso19115/2003/extent#GeographicBoundingBox> rdfs:subClassOf _:genid15 .

_:genid15 a owl:Restriction ;
	owl:onProperty <http://def.seegrid.csiro.au/isotc211/iso19115/2003/extent#northBoundLatitude> ;
	owl:cardinality "1"^^xsd:nonNegativeInteger .

<http://def.seegrid.csiro.au/isotc211/iso19115/2003/extent#GeographicBoundingBox> rdfs:subClassOf _:genid16 .

_:genid16 a owl:Restriction ;
	owl:onProperty <http://def.seegrid.csiro.au/isotc211/iso19115/2003/extent#southBoundLatitude> ;
	owl:cardinality "1"^^xsd:nonNegativeInteger .

<http://def.seegrid.csiro.au/isotc211/iso19115/2003/extent#GeographicBoundingBox> rdfs:subClassOf _:genid17 .

_:genid17 a owl:Restriction ;
	owl:onProperty <http://def.seegrid.csiro.au/isotc211/iso19115/2003/extent#westBoundLongitude> ;
	owl:cardinality "1"^^xsd:nonNegativeInteger .

<http://def.seegrid.csiro.au/isotc211/iso19115/2003/extent#GeographicBoundingBox> rdfs:isDefinedBy <http://def.seegrid.csiro.au/isotc211/iso19115/2003/extent> ;
	rdfs:label "Geographic bounding box"^^xsd:string ;
	<http://www.w3.org/2004/02/skos/core#notation> "EX_GeographicBoundingBox"^^<http://def.seegrid.csiro.au/isotc211/iso19150/-2/2012/basic#ISOClassName> .
# 
# http://def.seegrid.csiro.au/isotc211/iso19115/2003/extent#GeographicExtent

<http://def.seegrid.csiro.au/isotc211/iso19115/2003/extent#GeographicExtent> a owl:Class .
# 
# http://lexvo.org/ontology#Language

<http://lexvo.org/ontology#Language> a owl:Class ;
	rdfs:comment "Idioma en el que se expresa el contenido de un recurso."@es ;
	rdfs:label "Idioma"@es .
# 
# http://purl.org/dc/dcam/VocabularyEncodingScheme

<http://purl.org/dc/dcam/VocabularyEncodingScheme> a owl:Class .
# 
# http://purl.org/dc/dcmitype/Collection

<http://purl.org/dc/dcmitype/Collection> a owl:Class .
# 
# http://purl.org/dc/dcmitype/Dataset

<http://purl.org/dc/dcmitype/Dataset> a owl:Class .
# 
# http://purl.org/dc/terms/Agent

dcterms:Agent a owl:Class .
# 
# http://purl.org/dc/terms/AgentClass

dcterms:AgentClass a owl:Class ;
	rdfs:subClassOf rdfs:Class .
# 
# http://purl.org/dc/terms/BibliographicResource

dcterms:BibliographicResource a owl:Class .
# 
# http://purl.org/dc/terms/FileFormat

dcterms:FileFormat a owl:Class ;
	rdfs:subClassOf dcterms:MediaType .
# 
# http://purl.org/dc/terms/Frequency

dcterms:Frequency a owl:Class .
# 
# http://purl.org/dc/terms/Jurisdiction

dcterms:Jurisdiction a owl:Class ;
	rdfs:subClassOf dcterms:LocationPeriodOrJurisdiction .
# 
# http://purl.org/dc/terms/LicenseDocument

dcterms:LicenseDocument a owl:Class ;
	rdfs:subClassOf dcterms:RightsStatement .
# 
# http://purl.org/dc/terms/LinguisticSystem

dcterms:LinguisticSystem a owl:Class .
# 
# http://purl.org/dc/terms/Location

dcterms:Location a owl:Class ;
	rdfs:subClassOf dcterms:LocationPeriodOrJurisdiction .
# 
# http://purl.org/dc/terms/LocationPeriodOrJurisdiction

dcterms:LocationPeriodOrJurisdiction a owl:Class .
# 
# http://purl.org/dc/terms/MediaType

dcterms:MediaType a owl:Class ;
	rdfs:subClassOf dcterms:MediaTypeOrExtent .
# 
# http://purl.org/dc/terms/MediaTypeOrExtent

dcterms:MediaTypeOrExtent a owl:Class .
# 
# http://purl.org/dc/terms/MethodOfAccrual

dcterms:MethodOfAccrual a owl:Class .
# 
# http://purl.org/dc/terms/MethodOfInstruction

dcterms:MethodOfInstruction a owl:Class .
# 
# http://purl.org/dc/terms/PeriodOfTime

dcterms:PeriodOfTime a owl:Class ;
	rdfs:subClassOf dcterms:LocationPeriodOrJurisdiction .
# 
# http://purl.org/dc/terms/PhysicalMedium

dcterms:PhysicalMedium a owl:Class ;
	rdfs:subClassOf dcterms:MediaType .
# 
# http://purl.org/dc/terms/PhysicalResource

dcterms:PhysicalResource a owl:Class .
# 
# http://purl.org/dc/terms/Policy

dcterms:Policy a owl:Class .
# 
# http://purl.org/dc/terms/ProvenanceStatement

dcterms:ProvenanceStatement a owl:Class .
# 
# http://purl.org/dc/terms/RightsStatement

dcterms:RightsStatement a owl:Class .
# 
# http://purl.org/dc/terms/SizeOrDuration

dcterms:SizeOrDuration a owl:Class ;
	rdfs:subClassOf dcterms:MediaTypeOrExtent .
# 
# http://purl.org/dc/terms/Standard

dcterms:Standard a owl:Class .
# 
# http://purl.org/spar/datacite/Identifier

<http://purl.org/spar/datacite/Identifier> a owl:Class ;
	rdfs:comment "Un identificador que identifica de forma única a una entidad - tal como una agencia de financiación, una persona y un recurso - que pertenece a un esquema particular, como los especificados por individuos de la clase datacite:IdentifierScheme."@es ;
	rdfs:label "identificador"@es .
# 
# http://rdfs.org/ns/void#Dataset

<http://rdfs.org/ns/void#Dataset> a owl:Class .
# 
# http://www.geonames.org/ontology#Feature

<http://www.geonames.org/ontology#Feature> a owl:Class .
# 
# http://www.w3.org/2004/02/skos/core#Concept

<http://www.w3.org/2004/02/skos/core#Concept> rdfs:comment "Un concepto SKOS puede entenderse como una idea, una noción o una unidad de pensamiento."@es ;
	rdfs:label "Concept" , "Concepto"@es .
# 
# http://www.w3.org/2006/time#Interval

<http://www.w3.org/2006/time#Interval> a owl:Class ;
	rdfs:comment "Entidad temporal con extensión o duración."@es ;
	rdfs:label "Intervalo de tiempo"@es .
# 
# http://www.w3.org/ns/dcat#Dataset

<http://www.w3.org/ns/dcat#Dataset> a owl:Class ;
	rdfs:subClassOf <http://purl.org/dc/dcmitype/Dataset> ;
	vann:usageNote """Cette classe représente le jeu de données publié par le fournisseur de données. Dans les cas où une distinction est nécessaire entre le jeu de donénes et son 
					  entrée dans le catalogue, la classe registre de données peut être utilisée pour ce dernier. """@fr , """Esta clase representa el conjunto de datos publicado por el editor del conjunto de datos. En los casos donde es necesaria una distinción entre el
					conjunto de datos y su entrada en el catálogo de datos"""@es , """This class represents the actual dataset as published by the dataset publisher. In 
          cases where a distinction between the actual dataset and its entry in the catalog is 
          necessary (because metadata such as modification date and maintainer might differ), the 
          catalog record class can be used for the latter."""@en , """Η κλάση αυτή αναπαριστά το σύνολο δεδομένων αυτό καθ'εαυτό, όπως έχει δημοσιευθεί από τον εκδότη.
          Σε περιπτώσεις όπου είναι απαραίτητος ο διαχωρισμός μεταξύ του συνόλου δεδομένων και της καταγραφής αυτού στον κατάλογο (γιατί μεταδεδομένα όπως η ημερομηνία αλλαγής και ο συντηρητής μπορεί να διαφέρουν) 
          η κλάση της καταγραφής καταλόγου μπορεί να χρησιμοποιηθεί για το τελευταίο."""@el , "このクラスは、データセットの公開者が公開する実際のデータセットを表わします。カタログ内の実際のデータセットとそのエントリーとの区別が必要な場合（修正日と維持者などのメタデータが異なるかもしれないので）は、後者にcatalog recordというクラスを使用できます。"@ja ;
	rdfs:comment "1つのエージェントによって公開またはキュレートされ、1つ以上の形式でアクセスまたはダウンロードできるデータの集合。"@ja , "A collection of data, published or curated by a single source, and available for access or download in one or more formats"@en , "Una colección de datos, publicados o conservados por una única fuente, y disponibles para acceder o descagar en uno o más formatos"@es , "Une collection de données, publiée ou élaborée par une seule source, et disponible pour accès ou téléchargement dans un ou plusieurs formats"@fr , "Μία συλλογή από δεδομένα, δημοσιευμένη ή επιμελημένη από μία και μόνο πηγή, διαθέσιμη δε προς πρόσβαση ή μεταφόρτωση σε μία ή περισσότερες μορφές"@el , "قائمة بيانات منشورة أو مجموعة من قبل مصدر ما و متاح الوصول إليها أو تحميلها"@ar ;
	rdfs:isDefinedBy <http://www.w3.org/TR/vocab-dcat/> ;
	rdfs:label "Conjunto de datos"@es , "Dataset"@en , "Jeu de données"@fr , "Σύνολο Δεδομένων"@el , "قائمة بيانات"@ar , "データセット"@ja .
# 
# http://www.w3.org/ns/odrl/2/Policy

<http://www.w3.org/ns/odrl/2/Policy> a owl:Class ;
	rdfs:comment "Un grupo no vacio de permisos y/o prohibiciones."@es ;
	rdfs:label "Política de uso"@es .
# 
# http://www.w3.org/ns/prov#Entity

prov:Entity a owl:Class .
# 
# http://xmlns.com/foaf/0.1/Project

foaf:Project rdfs:comment "Un proyecto (un esfuerzo colectivo de algún tipo)."@es ;
	rdfs:label "Proyecto"@es .
# 
# https://w3id.org/def/inia#Dataset

<https://w3id.org/def/inia#Dataset> a owl:Class ;
	rdfs:subClassOf <http://dataid.dbpedia.org/ns/core#Dataset> , <https://w3id.org/def/inia#Resource> , _:genid18 .

_:genid18 a owl:Restriction ;
	owl:onProperty dcterms:creator ;
	owl:minCardinality "1"^^xsd:nonNegativeInteger .

<https://w3id.org/def/inia#Dataset> rdfs:subClassOf _:genid19 .

_:genid19 a owl:Restriction ;
	owl:onProperty dcterms:publisher ;
	owl:minQualifiedCardinality "1"^^xsd:nonNegativeInteger ;
	owl:onClass <http://www.w3.org/ns/org#Organization> .

<https://w3id.org/def/inia#Dataset> rdfs:subClassOf _:genid20 .

_:genid20 a owl:Restriction ;
	owl:onProperty <http://www.w3.org/ns/dcat#theme> ;
	owl:minQualifiedCardinality "1"^^xsd:nonNegativeInteger ;
	owl:onClass <http://www.w3.org/2004/02/skos/core#Concept> .

<https://w3id.org/def/inia#Dataset> rdfs:subClassOf _:genid21 .

_:genid21 a owl:Restriction ;
	owl:onProperty dcterms:description ;
	owl:minCardinality "1"^^xsd:nonNegativeInteger .

<https://w3id.org/def/inia#Dataset> rdfs:subClassOf _:genid22 .

_:genid22 a owl:Restriction ;
	owl:onProperty dcterms:issued ;
	owl:minQualifiedCardinality "1"^^xsd:nonNegativeInteger ;
	owl:onDataRange xsd:date .

<https://w3id.org/def/inia#Dataset> rdfs:subClassOf _:genid23 .

_:genid23 a owl:Restriction ;
	owl:onProperty dcterms:title ;
	owl:minCardinality "1"^^xsd:nonNegativeInteger .

<https://w3id.org/def/inia#Dataset> rdfs:comment "Dataset definido en la ontología INIA. Este dataset tendrá propiedades particulares de los metadatos manejados en los conjuntos de datos INIA."@es ;
	rdfs:label "Conjunto de datos"@es , "Dataset"@en .
# 
# https://w3id.org/def/inia#Resource

<https://w3id.org/def/inia#Resource> a owl:Class ;
	rdfs:label "Resource"@en .
# 
# 
# 
# #################################################################
# #
# #    Individuals
# #
# #################################################################
# 
# 
# http://dublincore.org/usage/terms/history/#Agent-001

<http://dublincore.org/usage/terms/history/#Agent-001> a owl:NamedIndividual .
# 
# http://dublincore.org/usage/terms/history/#AgentClass-003

<http://dublincore.org/usage/terms/history/#AgentClass-003> a owl:NamedIndividual .
# 
# http://dublincore.org/usage/terms/history/#BibliographicResource-001

<http://dublincore.org/usage/terms/history/#BibliographicResource-001> a owl:NamedIndividual .
# 
# http://dublincore.org/usage/terms/history/#Box-003

<http://dublincore.org/usage/terms/history/#Box-003> a owl:NamedIndividual .
# 
# http://dublincore.org/usage/terms/history/#DCMIType-005

<http://dublincore.org/usage/terms/history/#DCMIType-005> a owl:NamedIndividual .
# 
# http://dublincore.org/usage/terms/history/#DDC-003

<http://dublincore.org/usage/terms/history/#DDC-003> a owl:NamedIndividual .
# 
# http://dublincore.org/usage/terms/history/#FileFormat-001

<http://dublincore.org/usage/terms/history/#FileFormat-001> a owl:NamedIndividual .
# 
# http://dublincore.org/usage/terms/history/#Frequency-001

<http://dublincore.org/usage/terms/history/#Frequency-001> a owl:NamedIndividual .
# 
# http://dublincore.org/usage/terms/history/#IMT-004

<http://dublincore.org/usage/terms/history/#IMT-004> a owl:NamedIndividual .
# 
# http://dublincore.org/usage/terms/history/#ISO3166-004

<http://dublincore.org/usage/terms/history/#ISO3166-004> a owl:NamedIndividual .
# 
# http://dublincore.org/usage/terms/history/#ISO639-2-003

<http://dublincore.org/usage/terms/history/#ISO639-2-003> a owl:NamedIndividual .
# 
# http://dublincore.org/usage/terms/history/#ISO639-3-001

<http://dublincore.org/usage/terms/history/#ISO639-3-001> a owl:NamedIndividual .
# 
# http://dublincore.org/usage/terms/history/#Jurisdiction-001

<http://dublincore.org/usage/terms/history/#Jurisdiction-001> a owl:NamedIndividual .
# 
# http://dublincore.org/usage/terms/history/#LCC-003

<http://dublincore.org/usage/terms/history/#LCC-003> a owl:NamedIndividual .
# 
# http://dublincore.org/usage/terms/history/#LCSH-003

<http://dublincore.org/usage/terms/history/#LCSH-003> a owl:NamedIndividual .
# 
# http://dublincore.org/usage/terms/history/#LicenseDocument-001

<http://dublincore.org/usage/terms/history/#LicenseDocument-001> a owl:NamedIndividual .
# 
# http://dublincore.org/usage/terms/history/#LinguisticSystem-001

<http://dublincore.org/usage/terms/history/#LinguisticSystem-001> a owl:NamedIndividual .
# 
# http://dublincore.org/usage/terms/history/#Location-001

<http://dublincore.org/usage/terms/history/#Location-001> a owl:NamedIndividual .
# 
# http://dublincore.org/usage/terms/history/#LocationPeriodOrJurisdiction-001

<http://dublincore.org/usage/terms/history/#LocationPeriodOrJurisdiction-001> a owl:NamedIndividual .
# 
# http://dublincore.org/usage/terms/history/#MESH-003

<http://dublincore.org/usage/terms/history/#MESH-003> a owl:NamedIndividual .
# 
# http://dublincore.org/usage/terms/history/#MediaType-001

<http://dublincore.org/usage/terms/history/#MediaType-001> a owl:NamedIndividual .
# 
# http://dublincore.org/usage/terms/history/#MediaTypeOrExtent-001

<http://dublincore.org/usage/terms/history/#MediaTypeOrExtent-001> a owl:NamedIndividual .
# 
# http://dublincore.org/usage/terms/history/#MethodOfAccrual-001

<http://dublincore.org/usage/terms/history/#MethodOfAccrual-001> a owl:NamedIndividual .
# 
# http://dublincore.org/usage/terms/history/#MethodOfInstruction-001

<http://dublincore.org/usage/terms/history/#MethodOfInstruction-001> a owl:NamedIndividual .
# 
# http://dublincore.org/usage/terms/history/#NLM-002

<http://dublincore.org/usage/terms/history/#NLM-002> a owl:NamedIndividual .
# 
# http://dublincore.org/usage/terms/history/#Period-003

<http://dublincore.org/usage/terms/history/#Period-003> a owl:NamedIndividual .
# 
# http://dublincore.org/usage/terms/history/#PeriodOfTime-001

<http://dublincore.org/usage/terms/history/#PeriodOfTime-001> a owl:NamedIndividual .
# 
# http://dublincore.org/usage/terms/history/#PhysicalMedium-001

<http://dublincore.org/usage/terms/history/#PhysicalMedium-001> a owl:NamedIndividual .
# 
# http://dublincore.org/usage/terms/history/#PhysicalResource-001

<http://dublincore.org/usage/terms/history/#PhysicalResource-001> a owl:NamedIndividual .
# 
# http://dublincore.org/usage/terms/history/#Point-003

<http://dublincore.org/usage/terms/history/#Point-003> a owl:NamedIndividual .
# 
# http://dublincore.org/usage/terms/history/#Policy-001

<http://dublincore.org/usage/terms/history/#Policy-001> a owl:NamedIndividual .
# 
# http://dublincore.org/usage/terms/history/#ProvenanceStatement-001

<http://dublincore.org/usage/terms/history/#ProvenanceStatement-001> a owl:NamedIndividual .
# 
# http://dublincore.org/usage/terms/history/#RFC1766-003

<http://dublincore.org/usage/terms/history/#RFC1766-003> a owl:NamedIndividual .
# 
# http://dublincore.org/usage/terms/history/#RFC3066-002

<http://dublincore.org/usage/terms/history/#RFC3066-002> a owl:NamedIndividual .
# 
# http://dublincore.org/usage/terms/history/#RFC4646-001

<http://dublincore.org/usage/terms/history/#RFC4646-001> a owl:NamedIndividual .
# 
# http://dublincore.org/usage/terms/history/#RFC5646-001

<http://dublincore.org/usage/terms/history/#RFC5646-001> a owl:NamedIndividual .
# 
# http://dublincore.org/usage/terms/history/#RightsStatement-001

<http://dublincore.org/usage/terms/history/#RightsStatement-001> a owl:NamedIndividual .
# 
# http://dublincore.org/usage/terms/history/#SizeOrDuration-001

<http://dublincore.org/usage/terms/history/#SizeOrDuration-001> a owl:NamedIndividual .
# 
# http://dublincore.org/usage/terms/history/#Standard-001

<http://dublincore.org/usage/terms/history/#Standard-001> a owl:NamedIndividual .
# 
# http://dublincore.org/usage/terms/history/#TGN-003

<http://dublincore.org/usage/terms/history/#TGN-003> a owl:NamedIndividual .
# 
# http://dublincore.org/usage/terms/history/#UDC-003

<http://dublincore.org/usage/terms/history/#UDC-003> a owl:NamedIndividual .
# 
# http://dublincore.org/usage/terms/history/#URI-003

<http://dublincore.org/usage/terms/history/#URI-003> a owl:NamedIndividual .
# 
# http://dublincore.org/usage/terms/history/#W3CDTF-003

<http://dublincore.org/usage/terms/history/#W3CDTF-003> a owl:NamedIndividual .
# 
# http://dublincore.org/usage/terms/history/#abstract-003

<http://dublincore.org/usage/terms/history/#abstract-003> a owl:NamedIndividual .
# 
# http://dublincore.org/usage/terms/history/#accessRights-002

<http://dublincore.org/usage/terms/history/#accessRights-002> a owl:NamedIndividual .
# 
# http://dublincore.org/usage/terms/history/#accrualMethod-003

<http://dublincore.org/usage/terms/history/#accrualMethod-003> a owl:NamedIndividual .
# 
# http://dublincore.org/usage/terms/history/#accrualPeriodicity-003

<http://dublincore.org/usage/terms/history/#accrualPeriodicity-003> a owl:NamedIndividual .
# 
# http://dublincore.org/usage/terms/history/#accrualPolicy-003

<http://dublincore.org/usage/terms/history/#accrualPolicy-003> a owl:NamedIndividual .
# 
# http://dublincore.org/usage/terms/history/#alternative-003

<http://dublincore.org/usage/terms/history/#alternative-003> a owl:NamedIndividual .
# 
# http://dublincore.org/usage/terms/history/#audience-003

<http://dublincore.org/usage/terms/history/#audience-003> a owl:NamedIndividual .
# 
# http://dublincore.org/usage/terms/history/#available-003

<http://dublincore.org/usage/terms/history/#available-003> a owl:NamedIndividual .
# 
# http://dublincore.org/usage/terms/history/#bibliographicCitation-002

<http://dublincore.org/usage/terms/history/#bibliographicCitation-002> a owl:NamedIndividual .
# 
# http://dublincore.org/usage/terms/history/#conformsTo-003

<http://dublincore.org/usage/terms/history/#conformsTo-003> a owl:NamedIndividual .
# 
# http://dublincore.org/usage/terms/history/#contributorT-001

<http://dublincore.org/usage/terms/history/#contributorT-001> a owl:NamedIndividual .
# 
# http://dublincore.org/usage/terms/history/#coverageT-001

<http://dublincore.org/usage/terms/history/#coverageT-001> a owl:NamedIndividual .
# 
# http://dublincore.org/usage/terms/history/#created-003

<http://dublincore.org/usage/terms/history/#created-003> a owl:NamedIndividual .
# 
# http://dublincore.org/usage/terms/history/#creatorT-002

<http://dublincore.org/usage/terms/history/#creatorT-002> a owl:NamedIndividual .
# 
# http://dublincore.org/usage/terms/history/#dateAccepted-002

<http://dublincore.org/usage/terms/history/#dateAccepted-002> a owl:NamedIndividual .
# 
# http://dublincore.org/usage/terms/history/#dateCopyrighted-002

<http://dublincore.org/usage/terms/history/#dateCopyrighted-002> a owl:NamedIndividual .
# 
# http://dublincore.org/usage/terms/history/#dateSubmitted-002

<http://dublincore.org/usage/terms/history/#dateSubmitted-002> a owl:NamedIndividual .
# 
# http://dublincore.org/usage/terms/history/#dateT-001

<http://dublincore.org/usage/terms/history/#dateT-001> a owl:NamedIndividual .
# 
# http://dublincore.org/usage/terms/history/#descriptionT-001

<http://dublincore.org/usage/terms/history/#descriptionT-001> a owl:NamedIndividual .
# 
# http://dublincore.org/usage/terms/history/#educationLevel-002

<http://dublincore.org/usage/terms/history/#educationLevel-002> a owl:NamedIndividual .
# 
# http://dublincore.org/usage/terms/history/#extent-003

<http://dublincore.org/usage/terms/history/#extent-003> a owl:NamedIndividual .
# 
# http://dublincore.org/usage/terms/history/#formatT-001

<http://dublincore.org/usage/terms/history/#formatT-001> a owl:NamedIndividual .
# 
# http://dublincore.org/usage/terms/history/#hasFormat-003

<http://dublincore.org/usage/terms/history/#hasFormat-003> a owl:NamedIndividual .
# 
# http://dublincore.org/usage/terms/history/#hasPart-003

<http://dublincore.org/usage/terms/history/#hasPart-003> a owl:NamedIndividual .
# 
# http://dublincore.org/usage/terms/history/#hasVersion-003

<http://dublincore.org/usage/terms/history/#hasVersion-003> a owl:NamedIndividual .
# 
# http://dublincore.org/usage/terms/history/#identifierT-001

<http://dublincore.org/usage/terms/history/#identifierT-001> a owl:NamedIndividual .
# 
# http://dublincore.org/usage/terms/history/#instructionalMethod-002

<http://dublincore.org/usage/terms/history/#instructionalMethod-002> a owl:NamedIndividual .
# 
# http://dublincore.org/usage/terms/history/#isFormatOf-003

<http://dublincore.org/usage/terms/history/#isFormatOf-003> a owl:NamedIndividual .
# 
# http://dublincore.org/usage/terms/history/#isPartOf-003

<http://dublincore.org/usage/terms/history/#isPartOf-003> a owl:NamedIndividual .
# 
# http://dublincore.org/usage/terms/history/#isReferencedBy-003

<http://dublincore.org/usage/terms/history/#isReferencedBy-003> a owl:NamedIndividual .
# 
# http://dublincore.org/usage/terms/history/#isReplacedBy-003

<http://dublincore.org/usage/terms/history/#isReplacedBy-003> a owl:NamedIndividual .
# 
# http://dublincore.org/usage/terms/history/#isRequiredBy-003

<http://dublincore.org/usage/terms/history/#isRequiredBy-003> a owl:NamedIndividual .
# 
# http://dublincore.org/usage/terms/history/#isVersionOf-003

<http://dublincore.org/usage/terms/history/#isVersionOf-003> a owl:NamedIndividual .
# 
# http://dublincore.org/usage/terms/history/#issued-003

<http://dublincore.org/usage/terms/history/#issued-003> a owl:NamedIndividual .
# 
# http://dublincore.org/usage/terms/history/#languageT-001

<http://dublincore.org/usage/terms/history/#languageT-001> a owl:NamedIndividual .
# 
# http://dublincore.org/usage/terms/history/#license-002

<http://dublincore.org/usage/terms/history/#license-002> a owl:NamedIndividual .
# 
# http://dublincore.org/usage/terms/history/#mediator-003

<http://dublincore.org/usage/terms/history/#mediator-003> a owl:NamedIndividual .
# 
# http://dublincore.org/usage/terms/history/#medium-003

<http://dublincore.org/usage/terms/history/#medium-003> a owl:NamedIndividual .
# 
# http://dublincore.org/usage/terms/history/#modified-003

<http://dublincore.org/usage/terms/history/#modified-003> a owl:NamedIndividual .
# 
# http://dublincore.org/usage/terms/history/#provenance-002

<http://dublincore.org/usage/terms/history/#provenance-002> a owl:NamedIndividual .
# 
# http://dublincore.org/usage/terms/history/#publisherT-001

<http://dublincore.org/usage/terms/history/#publisherT-001> a owl:NamedIndividual .
# 
# http://dublincore.org/usage/terms/history/#references-003

<http://dublincore.org/usage/terms/history/#references-003> a owl:NamedIndividual .
# 
# http://dublincore.org/usage/terms/history/#relationT-001

<http://dublincore.org/usage/terms/history/#relationT-001> a owl:NamedIndividual .
# 
# http://dublincore.org/usage/terms/history/#replaces-003

<http://dublincore.org/usage/terms/history/#replaces-003> a owl:NamedIndividual .
# 
# http://dublincore.org/usage/terms/history/#requires-003

<http://dublincore.org/usage/terms/history/#requires-003> a owl:NamedIndividual .
# 
# http://dublincore.org/usage/terms/history/#rightsHolder-002

<http://dublincore.org/usage/terms/history/#rightsHolder-002> a owl:NamedIndividual .
# 
# http://dublincore.org/usage/terms/history/#rightsT-001

<http://dublincore.org/usage/terms/history/#rightsT-001> a owl:NamedIndividual .
# 
# http://dublincore.org/usage/terms/history/#sourceT-001

<http://dublincore.org/usage/terms/history/#sourceT-001> a owl:NamedIndividual .
# 
# http://dublincore.org/usage/terms/history/#spatial-003

<http://dublincore.org/usage/terms/history/#spatial-003> a owl:NamedIndividual .
# 
# http://dublincore.org/usage/terms/history/#subjectT-002

<http://dublincore.org/usage/terms/history/#subjectT-002> a owl:NamedIndividual .
# 
# http://dublincore.org/usage/terms/history/#tableOfContents-003

<http://dublincore.org/usage/terms/history/#tableOfContents-003> a owl:NamedIndividual .
# 
# http://dublincore.org/usage/terms/history/#temporal-003

<http://dublincore.org/usage/terms/history/#temporal-003> a owl:NamedIndividual .
# 
# http://dublincore.org/usage/terms/history/#titleT-002

<http://dublincore.org/usage/terms/history/#titleT-002> a owl:NamedIndividual .
# 
# http://dublincore.org/usage/terms/history/#typeT-001

<http://dublincore.org/usage/terms/history/#typeT-001> a owl:NamedIndividual .
# 
# http://dublincore.org/usage/terms/history/#valid-003

<http://dublincore.org/usage/terms/history/#valid-003> a owl:NamedIndividual .
# 
# http://purl.org/dc/aboutdcmi#DCMI

<http://purl.org/dc/aboutdcmi#DCMI> a owl:NamedIndividual .
# 
# http://purl.org/dc/terms/

<http://purl.org/dc/terms/> a owl:NamedIndividual ;
	dcterms:modified "2012-06-14"^^xsd:date ;
	dcterms:publisher <http://purl.org/dc/aboutdcmi#DCMI> ;
	dcterms:title "DCMI Metadata Terms - other"@en .
# 
# http://purl.org/dc/terms/Agent

dcterms:Agent a owl:NamedIndividual , dcterms:AgentClass .
# 
# http://purl.org/dc/terms/AgentClass

dcterms:AgentClass a owl:NamedIndividual .
# 
# http://purl.org/dc/terms/BibliographicResource

dcterms:BibliographicResource a owl:NamedIndividual .
# 
# http://purl.org/dc/terms/Box

dcterms:Box a owl:NamedIndividual .
# 
# http://purl.org/dc/terms/DCMIType

dcterms:DCMIType a owl:NamedIndividual , <http://purl.org/dc/dcam/VocabularyEncodingScheme> ;
	dcterms:hasVersion <http://dublincore.org/usage/terms/history/#DCMIType-005> ;
	dcterms:issued "2000-07-11"^^xsd:date ;
	dcterms:modified "2012-06-14"^^xsd:date ;
	rdfs:comment "The set of classes specified by the DCMI Type Vocabulary, used to categorize the nature or genre of the resource."@en ;
	rdfs:isDefinedBy <http://purl.org/dc/terms/> ;
	rdfs:label "DCMI Type Vocabulary"@en ;
	rdfs:seeAlso <http://purl.org/dc/dcmitype/> .
# 
# http://purl.org/dc/terms/DDC

dcterms:DDC a owl:NamedIndividual , <http://purl.org/dc/dcam/VocabularyEncodingScheme> ;
	dcterms:hasVersion <http://dublincore.org/usage/terms/history/#DDC-003> ;
	dcterms:issued "2000-07-11"^^xsd:date ;
	dcterms:modified "2008-01-14"^^xsd:date ;
	rdfs:comment "The set of conceptual resources specified by the Dewey Decimal Classification."@en ;
	rdfs:isDefinedBy <http://purl.org/dc/terms/> ;
	rdfs:label "DDC"@en ;
	rdfs:seeAlso <http://www.oclc.org/dewey/> .
# 
# http://purl.org/dc/terms/FileFormat

dcterms:FileFormat a owl:NamedIndividual .
# 
# http://purl.org/dc/terms/Frequency

dcterms:Frequency a owl:NamedIndividual .
# 
# http://purl.org/dc/terms/IMT

dcterms:IMT a owl:NamedIndividual , <http://purl.org/dc/dcam/VocabularyEncodingScheme> ;
	dcterms:hasVersion <http://dublincore.org/usage/terms/history/#IMT-004> ;
	dcterms:issued "2000-07-11"^^xsd:date ;
	dcterms:modified "2008-01-14"^^xsd:date ;
	rdfs:comment "The set of media types specified by the Internet Assigned Numbers Authority."@en ;
	rdfs:isDefinedBy <http://purl.org/dc/terms/> ;
	rdfs:label "IMT"@en ;
	rdfs:seeAlso <http://www.iana.org/assignments/media-types/> .
# 
# http://purl.org/dc/terms/ISO3166

dcterms:ISO3166 a owl:NamedIndividual .
# 
# http://purl.org/dc/terms/ISO639-2

dcterms:ISO639-2 a owl:NamedIndividual .
# 
# http://purl.org/dc/terms/ISO639-3

dcterms:ISO639-3 a owl:NamedIndividual .
# 
# http://purl.org/dc/terms/Jurisdiction

dcterms:Jurisdiction a owl:NamedIndividual .
# 
# http://purl.org/dc/terms/LCC

dcterms:LCC a owl:NamedIndividual , <http://purl.org/dc/dcam/VocabularyEncodingScheme> ;
	dcterms:hasVersion <http://dublincore.org/usage/terms/history/#LCC-003> ;
	dcterms:issued "2000-07-11"^^xsd:date ;
	dcterms:modified "2008-01-14"^^xsd:date ;
	rdfs:comment "The set of conceptual resources specified by the Library of Congress Classification."@en ;
	rdfs:isDefinedBy <http://purl.org/dc/terms/> ;
	rdfs:label "LCC"@en ;
	rdfs:seeAlso <http://lcweb.loc.gov/catdir/cpso/lcco/lcco.html> .
# 
# http://purl.org/dc/terms/LCSH

dcterms:LCSH a owl:NamedIndividual , <http://purl.org/dc/dcam/VocabularyEncodingScheme> ;
	dcterms:hasVersion <http://dublincore.org/usage/terms/history/#LCSH-003> ;
	dcterms:issued "2000-07-11"^^xsd:date ;
	dcterms:modified "2008-01-14"^^xsd:date ;
	rdfs:comment "The set of labeled concepts specified by the Library of Congress Subject Headings."@en ;
	rdfs:isDefinedBy <http://purl.org/dc/terms/> ;
	rdfs:label "LCSH"@en .
# 
# http://purl.org/dc/terms/LicenseDocument

dcterms:LicenseDocument a owl:NamedIndividual .
# 
# http://purl.org/dc/terms/LinguisticSystem

dcterms:LinguisticSystem a owl:NamedIndividual .
# 
# http://purl.org/dc/terms/Location

dcterms:Location a owl:NamedIndividual .
# 
# http://purl.org/dc/terms/LocationPeriodOrJurisdiction

dcterms:LocationPeriodOrJurisdiction a owl:NamedIndividual .
# 
# http://purl.org/dc/terms/MESH

dcterms:MESH a owl:NamedIndividual , <http://purl.org/dc/dcam/VocabularyEncodingScheme> ;
	dcterms:hasVersion <http://dublincore.org/usage/terms/history/#MESH-003> ;
	dcterms:issued "2000-07-11"^^xsd:date ;
	dcterms:modified "2008-01-14"^^xsd:date ;
	rdfs:comment "The set of labeled concepts specified by the Medical Subject Headings."@en ;
	rdfs:isDefinedBy <http://purl.org/dc/terms/> ;
	rdfs:label "MeSH"@en ;
	rdfs:seeAlso <http://www.nlm.nih.gov/mesh/meshhome.html> .
# 
# http://purl.org/dc/terms/MediaType

dcterms:MediaType a owl:NamedIndividual .
# 
# http://purl.org/dc/terms/MediaTypeOrExtent

dcterms:MediaTypeOrExtent a owl:NamedIndividual .
# 
# http://purl.org/dc/terms/MethodOfAccrual

dcterms:MethodOfAccrual a owl:NamedIndividual .
# 
# http://purl.org/dc/terms/MethodOfInstruction

dcterms:MethodOfInstruction a owl:NamedIndividual .
# 
# http://purl.org/dc/terms/NLM

dcterms:NLM a owl:NamedIndividual , <http://purl.org/dc/dcam/VocabularyEncodingScheme> ;
	dcterms:hasVersion <http://dublincore.org/usage/terms/history/#NLM-002> ;
	dcterms:issued "2005-06-13"^^xsd:date ;
	dcterms:modified "2008-01-14"^^xsd:date ;
	rdfs:comment "The set of conceptual resources specified by the National Library of Medicine Classification."@en ;
	rdfs:isDefinedBy <http://purl.org/dc/terms/> ;
	rdfs:label "NLM"@en ;
	rdfs:seeAlso <http://wwwcf.nlm.nih.gov/class/> .
# 
# http://purl.org/dc/terms/Period

dcterms:Period a owl:NamedIndividual .
# 
# http://purl.org/dc/terms/PeriodOfTime

dcterms:PeriodOfTime a owl:NamedIndividual .
# 
# http://purl.org/dc/terms/PhysicalMedium

dcterms:PhysicalMedium a owl:NamedIndividual .
# 
# http://purl.org/dc/terms/PhysicalResource

dcterms:PhysicalResource a owl:NamedIndividual .
# 
# http://purl.org/dc/terms/Point

dcterms:Point a owl:NamedIndividual .
# 
# http://purl.org/dc/terms/Policy

dcterms:Policy a owl:NamedIndividual .
# 
# http://purl.org/dc/terms/ProvenanceStatement

dcterms:ProvenanceStatement a owl:NamedIndividual .
# 
# http://purl.org/dc/terms/RFC1766

dcterms:RFC1766 a owl:NamedIndividual .
# 
# http://purl.org/dc/terms/RFC3066

dcterms:RFC3066 a owl:NamedIndividual .
# 
# http://purl.org/dc/terms/RFC4646

dcterms:RFC4646 a owl:NamedIndividual .
# 
# http://purl.org/dc/terms/RFC5646

dcterms:RFC5646 a owl:NamedIndividual .
# 
# http://purl.org/dc/terms/RightsStatement

dcterms:RightsStatement a owl:NamedIndividual .
# 
# http://purl.org/dc/terms/SizeOrDuration

dcterms:SizeOrDuration a owl:NamedIndividual .
# 
# http://purl.org/dc/terms/Standard

dcterms:Standard a owl:NamedIndividual .
# 
# http://purl.org/dc/terms/TGN

dcterms:TGN a owl:NamedIndividual , <http://purl.org/dc/dcam/VocabularyEncodingScheme> ;
	dcterms:hasVersion <http://dublincore.org/usage/terms/history/#TGN-003> ;
	dcterms:issued "2000-07-11"^^xsd:date ;
	dcterms:modified "2008-01-14"^^xsd:date ;
	rdfs:comment "The set of places specified by the Getty Thesaurus of Geographic Names."@en ;
	rdfs:isDefinedBy <http://purl.org/dc/terms/> ;
	rdfs:label "TGN"@en ;
	rdfs:seeAlso <http://www.getty.edu/research/tools/vocabulary/tgn/index.html> .
# 
# http://purl.org/dc/terms/UDC

dcterms:UDC a owl:NamedIndividual , <http://purl.org/dc/dcam/VocabularyEncodingScheme> ;
	dcterms:hasVersion <http://dublincore.org/usage/terms/history/#UDC-003> ;
	dcterms:issued "2000-07-11"^^xsd:date ;
	dcterms:modified "2008-01-14"^^xsd:date ;
	rdfs:comment "The set of conceptual resources specified by the Universal Decimal Classification."@en ;
	rdfs:isDefinedBy <http://purl.org/dc/terms/> ;
	rdfs:label "UDC"@en ;
	rdfs:seeAlso <http://www.udcc.org/> .
# 
# http://purl.org/dc/terms/URI

dcterms:URI a owl:NamedIndividual .
# 
# http://purl.org/dc/terms/W3CDTF

dcterms:W3CDTF a owl:NamedIndividual .
# 
# http://purl.org/dc/terms/abstract

dcterms:abstract a owl:NamedIndividual .
# 
# http://purl.org/dc/terms/accessRights

dcterms:accessRights a owl:NamedIndividual .
# 
# http://purl.org/dc/terms/accrualMethod

dcterms:accrualMethod a owl:NamedIndividual .
# 
# http://purl.org/dc/terms/accrualPeriodicity

dcterms:accrualPeriodicity a owl:NamedIndividual .
# 
# http://purl.org/dc/terms/accrualPolicy

dcterms:accrualPolicy a owl:NamedIndividual .
# 
# http://purl.org/dc/terms/alternative

dcterms:alternative a owl:NamedIndividual .
# 
# http://purl.org/dc/terms/audience

dcterms:audience a owl:NamedIndividual .
# 
# http://purl.org/dc/terms/available

dcterms:available a owl:NamedIndividual .
# 
# http://purl.org/dc/terms/bibliographicCitation

dcterms:bibliographicCitation a owl:NamedIndividual .
# 
# http://purl.org/dc/terms/conformsTo

dcterms:conformsTo a owl:NamedIndividual .
# 
# http://purl.org/dc/terms/contributor

dcterms:contributor a owl:NamedIndividual .
# 
# http://purl.org/dc/terms/coverage

dcterms:coverage a owl:NamedIndividual .
# 
# http://purl.org/dc/terms/created

dcterms:created a owl:NamedIndividual .
# 
# http://purl.org/dc/terms/creator

dcterms:creator a owl:NamedIndividual .
# 
# http://purl.org/dc/terms/date

dcterms:date a owl:NamedIndividual .
# 
# http://purl.org/dc/terms/dateAccepted

dcterms:dateAccepted a owl:NamedIndividual .
# 
# http://purl.org/dc/terms/dateCopyrighted

dcterms:dateCopyrighted a owl:NamedIndividual .
# 
# http://purl.org/dc/terms/dateSubmitted

dcterms:dateSubmitted a owl:NamedIndividual .
# 
# http://purl.org/dc/terms/description

dcterms:description a owl:NamedIndividual .
# 
# http://purl.org/dc/terms/educationLevel

dcterms:educationLevel a owl:NamedIndividual .
# 
# http://purl.org/dc/terms/extent

dcterms:extent a owl:NamedIndividual .
# 
# http://purl.org/dc/terms/format

dcterms:format a owl:NamedIndividual .
# 
# http://purl.org/dc/terms/hasFormat

dcterms:hasFormat a owl:NamedIndividual .
# 
# http://purl.org/dc/terms/hasPart

dcterms:hasPart a owl:NamedIndividual .
# 
# http://purl.org/dc/terms/hasVersion

dcterms:hasVersion a owl:NamedIndividual .
# 
# http://purl.org/dc/terms/identifier

dcterms:identifier a owl:NamedIndividual .
# 
# http://purl.org/dc/terms/instructionalMethod

dcterms:instructionalMethod a owl:NamedIndividual .
# 
# http://purl.org/dc/terms/isFormatOf

dcterms:isFormatOf a owl:NamedIndividual .
# 
# http://purl.org/dc/terms/isPartOf

dcterms:isPartOf a owl:NamedIndividual .
# 
# http://purl.org/dc/terms/isReferencedBy

dcterms:isReferencedBy a owl:NamedIndividual .
# 
# http://purl.org/dc/terms/isReplacedBy

dcterms:isReplacedBy a owl:NamedIndividual .
# 
# http://purl.org/dc/terms/isRequiredBy

dcterms:isRequiredBy a owl:NamedIndividual .
# 
# http://purl.org/dc/terms/isVersionOf

dcterms:isVersionOf a owl:NamedIndividual .
# 
# http://purl.org/dc/terms/issued

dcterms:issued a owl:NamedIndividual .
# 
# http://purl.org/dc/terms/language

dcterms:language a owl:NamedIndividual .
# 
# http://purl.org/dc/terms/license

dcterms:license a owl:NamedIndividual .
# 
# http://purl.org/dc/terms/mediator

dcterms:mediator a owl:NamedIndividual .
# 
# http://purl.org/dc/terms/medium

dcterms:medium a owl:NamedIndividual .
# 
# http://purl.org/dc/terms/modified

dcterms:modified a owl:NamedIndividual .
# 
# http://purl.org/dc/terms/provenance

dcterms:provenance a owl:NamedIndividual .
# 
# http://purl.org/dc/terms/publisher

dcterms:publisher a owl:NamedIndividual .
# 
# http://purl.org/dc/terms/references

dcterms:references a owl:NamedIndividual .
# 
# http://purl.org/dc/terms/relation

dcterms:relation a owl:NamedIndividual .
# 
# http://purl.org/dc/terms/replaces

dcterms:replaces a owl:NamedIndividual .
# 
# http://purl.org/dc/terms/requires

dcterms:requires a owl:NamedIndividual .
# 
# http://purl.org/dc/terms/rights

dcterms:rights a owl:NamedIndividual .
# 
# http://purl.org/dc/terms/rightsHolder

dcterms:rightsHolder a owl:NamedIndividual .
# 
# http://purl.org/dc/terms/source

dcterms:source a owl:NamedIndividual .
# 
# http://purl.org/dc/terms/spatial

dcterms:spatial a owl:NamedIndividual .
# 
# http://purl.org/dc/terms/subject

dcterms:subject a owl:NamedIndividual .
# 
# http://purl.org/dc/terms/tableOfContents

dcterms:tableOfContents a owl:NamedIndividual .
# 
# http://purl.org/dc/terms/temporal

dcterms:temporal a owl:NamedIndividual .
# 
# http://purl.org/dc/terms/title

dcterms:title a owl:NamedIndividual .
# 
# http://purl.org/dc/terms/type

dcterms:type a owl:NamedIndividual .
# 
# http://purl.org/dc/terms/valid

dcterms:valid a owl:NamedIndividual .
# 
# http://purl.org/net/mpoveda

<http://purl.org/net/mpoveda> a owl:NamedIndividual .
# 
# 
# 
# #################################################################
# #
# #    Annotations
# #
# #################################################################
# 
# 

dcterms:Agent rdfs:label "Agent"@en ;
	rdfs:isDefinedBy <http://purl.org/dc/terms/> ;
	rdfs:comment "A resource that acts or has the power to act."@en ;
	dcterms:issued "2008-01-14"^^xsd:date ;
	dcterms:description "Examples of Agent include person, organization, and software agent."@en ;
	dcterms:hasVersion <http://dublincore.org/usage/terms/history/#Agent-001> .
# 

dcterms:AgentClass dcterms:issued "2008-01-14"^^xsd:date ;
	rdfs:isDefinedBy <http://purl.org/dc/terms/> ;
	rdfs:label "Agent Class"@en ;
	rdfs:comment "A group of agents."@en ;
	dcterms:modified "2012-06-14"^^xsd:date ;
	dcterms:description "Examples of Agent Class include groups seen as classes, such as students, women, charities, lecturers."@en ;
	dcterms:hasVersion <http://dublincore.org/usage/terms/history/#AgentClass-003> .
# 

dcterms:BibliographicResource rdfs:isDefinedBy <http://purl.org/dc/terms/> ;
	dcterms:hasVersion <http://dublincore.org/usage/terms/history/#BibliographicResource-001> ;
	rdfs:comment "A book, article, or other documentary resource."@en ;
	rdfs:label "Bibliographic Resource"@en ;
	dcterms:issued "2008-01-14"^^xsd:date .
# 

dcterms:Box dcterms:issued "2000-07-11"^^xsd:date ;
	rdfs:comment "The set of regions in space defined by their geographic coordinates according to the DCMI Box Encoding Scheme."@en ;
	rdfs:isDefinedBy <http://purl.org/dc/terms/> ;
	rdfs:seeAlso <http://dublincore.org/documents/dcmi-box/> ;
	dcterms:modified "2008-01-14"^^xsd:date ;
	rdfs:label "DCMI Box"@en ;
	dcterms:hasVersion <http://dublincore.org/usage/terms/history/#Box-003> .
# 

dcterms:FileFormat dcterms:description "Examples include the formats defined by the list of Internet Media Types."@en ;
	dcterms:hasVersion <http://dublincore.org/usage/terms/history/#FileFormat-001> ;
	rdfs:comment "A digital resource format."@en ;
	rdfs:label "File Format"@en ;
	dcterms:issued "2008-01-14"^^xsd:date ;
	rdfs:isDefinedBy <http://purl.org/dc/terms/> .
# 

dcterms:Frequency rdfs:label "Frequency"@en ;
	dcterms:hasVersion <http://dublincore.org/usage/terms/history/#Frequency-001> ;
	rdfs:isDefinedBy <http://purl.org/dc/terms/> ;
	rdfs:comment "A rate at which something recurs."@en ;
	dcterms:issued "2008-01-14"^^xsd:date .
# 

dcterms:ISO3166 dcterms:issued "2000-07-11"^^xsd:date ;
	rdfs:comment "The set of codes listed in ISO 3166-1 for the representation of names of countries."@en ;
	rdfs:isDefinedBy <http://purl.org/dc/terms/> ;
	dcterms:hasVersion <http://dublincore.org/usage/terms/history/#ISO3166-004> ;
	dcterms:modified "2008-01-14"^^xsd:date ;
	rdfs:label "ISO 3166"@en ;
	rdfs:seeAlso <http://www.iso.org/iso/en/prods-services/iso3166ma/02iso-3166-code-lists/list-en1.html> .
# 

dcterms:ISO639-2 rdfs:seeAlso <http://lcweb.loc.gov/standards/iso639-2/langhome.html> ;
	dcterms:modified "2008-01-14"^^xsd:date ;
	dcterms:issued "2000-07-11"^^xsd:date ;
	rdfs:comment "The three-letter alphabetic codes listed in ISO639-2 for the representation of names of languages."@en ;
	rdfs:isDefinedBy <http://purl.org/dc/terms/> ;
	rdfs:label "ISO 639-2"@en ;
	dcterms:hasVersion <http://dublincore.org/usage/terms/history/#ISO639-2-003> .
# 

dcterms:ISO639-3 rdfs:label "ISO 639-3"@en ;
	rdfs:comment "The set of three-letter codes listed in ISO 639-3 for the representation of names of languages."@en ;
	dcterms:hasVersion <http://dublincore.org/usage/terms/history/#ISO639-3-001> ;
	rdfs:isDefinedBy <http://purl.org/dc/terms/> ;
	dcterms:issued "2008-01-14"^^xsd:date ;
	rdfs:seeAlso <http://www.sil.org/iso639-3/> .
# 

dcterms:Jurisdiction dcterms:hasVersion <http://dublincore.org/usage/terms/history/#Jurisdiction-001> ;
	rdfs:label "Jurisdiction"@en ;
	dcterms:issued "2008-01-14"^^xsd:date ;
	rdfs:isDefinedBy <http://purl.org/dc/terms/> ;
	rdfs:comment "The extent or range of judicial, law enforcement, or other authority."@en .
# 

dcterms:LicenseDocument rdfs:isDefinedBy <http://purl.org/dc/terms/> ;
	rdfs:label "License Document"@en ;
	dcterms:issued "2008-01-14"^^xsd:date ;
	rdfs:comment "A legal document giving official permission to do something with a Resource."@en ;
	dcterms:hasVersion <http://dublincore.org/usage/terms/history/#LicenseDocument-001> .
# 

dcterms:LinguisticSystem dcterms:issued "2008-01-14"^^xsd:date ;
	dcterms:hasVersion <http://dublincore.org/usage/terms/history/#LinguisticSystem-001> ;
	dcterms:description "Examples include written, spoken, sign, and computer languages."@en ;
	rdfs:isDefinedBy <http://purl.org/dc/terms/> ;
	rdfs:comment "A system of signs, symbols, sounds, gestures, or rules used in communication."@en ;
	rdfs:label "Linguistic System"@en .
# 

dcterms:Location dcterms:hasVersion <http://dublincore.org/usage/terms/history/#Location-001> ;
	dcterms:issued "2008-01-14"^^xsd:date ;
	rdfs:label "Location"@en ;
	rdfs:isDefinedBy <http://purl.org/dc/terms/> ;
	rdfs:comment "A spatial region or named place."@en .
# 

dcterms:LocationPeriodOrJurisdiction rdfs:label "Location, Period, or Jurisdiction"@en ;
	dcterms:issued "2008-01-14"^^xsd:date ;
	rdfs:comment "A location, period of time, or jurisdiction."@en ;
	rdfs:isDefinedBy <http://purl.org/dc/terms/> ;
	dcterms:hasVersion <http://dublincore.org/usage/terms/history/#LocationPeriodOrJurisdiction-001> .
# 

dcterms:MediaType rdfs:comment "A file format or physical medium."@en ;
	rdfs:label "Media Type"@en ;
	rdfs:isDefinedBy <http://purl.org/dc/terms/> ;
	dcterms:hasVersion <http://dublincore.org/usage/terms/history/#MediaType-001> ;
	dcterms:issued "2008-01-14"^^xsd:date .
# 

dcterms:MediaTypeOrExtent rdfs:isDefinedBy <http://purl.org/dc/terms/> ;
	rdfs:comment "A media type or extent."@en ;
	rdfs:label "Media Type or Extent"@en ;
	dcterms:issued "2008-01-14"^^xsd:date ;
	dcterms:hasVersion <http://dublincore.org/usage/terms/history/#MediaTypeOrExtent-001> .
# 

dcterms:MethodOfAccrual rdfs:isDefinedBy <http://purl.org/dc/terms/> ;
	rdfs:comment "A method by which resources are added to a collection."@en ;
	dcterms:hasVersion <http://dublincore.org/usage/terms/history/#MethodOfAccrual-001> ;
	rdfs:label "Method of Accrual"@en ;
	dcterms:issued "2008-01-14"^^xsd:date .
# 

dcterms:MethodOfInstruction rdfs:label "Method of Instruction"@en ;
	rdfs:comment "A process that is used to engender knowledge, attitudes, and skills."@en ;
	rdfs:isDefinedBy <http://purl.org/dc/terms/> ;
	dcterms:hasVersion <http://dublincore.org/usage/terms/history/#MethodOfInstruction-001> ;
	dcterms:issued "2008-01-14"^^xsd:date .
# 

dcterms:Period rdfs:seeAlso <http://dublincore.org/documents/dcmi-period/> ;
	rdfs:comment "The set of time intervals defined by their limits according to the DCMI Period Encoding Scheme."@en ;
	dcterms:modified "2008-01-14"^^xsd:date ;
	dcterms:issued "2000-07-11"^^xsd:date ;
	rdfs:label "DCMI Period"@en ;
	rdfs:isDefinedBy <http://purl.org/dc/terms/> ;
	dcterms:hasVersion <http://dublincore.org/usage/terms/history/#Period-003> .
# 

dcterms:PeriodOfTime rdfs:comment "An interval of time that is named or defined by its start and end dates."@en ;
	dcterms:hasVersion <http://dublincore.org/usage/terms/history/#PeriodOfTime-001> ;
	rdfs:isDefinedBy <http://purl.org/dc/terms/> ;
	rdfs:label "Period of Time"@en ;
	dcterms:issued "2008-01-14"^^xsd:date .
# 

dcterms:PhysicalMedium dcterms:hasVersion <http://dublincore.org/usage/terms/history/#PhysicalMedium-001> ;
	dcterms:issued "2008-01-14"^^xsd:date ;
	dcterms:description "Examples include paper, canvas, or DVD."@en ;
	rdfs:isDefinedBy <http://purl.org/dc/terms/> ;
	rdfs:label "Physical Medium"@en ;
	rdfs:comment "A physical material or carrier."@en .
# 

dcterms:PhysicalResource rdfs:isDefinedBy <http://purl.org/dc/terms/> ;
	dcterms:issued "2008-01-14"^^xsd:date ;
	rdfs:comment "A material thing."@en ;
	dcterms:hasVersion <http://dublincore.org/usage/terms/history/#PhysicalResource-001> ;
	rdfs:label "Physical Resource"@en .
# 

dcterms:Point rdfs:comment "The set of points in space defined by their geographic coordinates according to the DCMI Point Encoding Scheme."@en ;
	rdfs:label "DCMI Point"@en ;
	dcterms:modified "2008-01-14"^^xsd:date ;
	dcterms:issued "2000-07-11"^^xsd:date ;
	dcterms:hasVersion <http://dublincore.org/usage/terms/history/#Point-003> ;
	rdfs:seeAlso <http://dublincore.org/documents/dcmi-point/> ;
	rdfs:isDefinedBy <http://purl.org/dc/terms/> .
# 

dcterms:Policy rdfs:isDefinedBy <http://purl.org/dc/terms/> ;
	rdfs:label "Policy"@en ;
	rdfs:comment "A plan or course of action by an authority, intended to influence and determine decisions, actions, and other matters."@en ;
	dcterms:hasVersion <http://dublincore.org/usage/terms/history/#Policy-001> ;
	dcterms:issued "2008-01-14"^^xsd:date .
# 

dcterms:ProvenanceStatement rdfs:label "Provenance Statement"@en ;
	rdfs:isDefinedBy <http://purl.org/dc/terms/> ;
	dcterms:issued "2008-01-14"^^xsd:date ;
	dcterms:hasVersion <http://dublincore.org/usage/terms/history/#ProvenanceStatement-001> ;
	rdfs:comment "A statement of any changes in ownership and custody of a resource since its creation that are significant for its authenticity, integrity, and interpretation."@en .
# 

dcterms:RFC1766 rdfs:isDefinedBy <http://purl.org/dc/terms/> ;
	dcterms:issued "2000-07-11"^^xsd:date ;
	dcterms:modified "2008-01-14"^^xsd:date ;
	dcterms:hasVersion <http://dublincore.org/usage/terms/history/#RFC1766-003> ;
	rdfs:comment "The set of tags, constructed according to RFC 1766, for the identification of languages."@en ;
	rdfs:seeAlso <http://www.ietf.org/rfc/rfc1766.txt> ;
	rdfs:label "RFC 1766"@en .
# 

dcterms:RFC3066 dcterms:issued "2002-07-13"^^xsd:date ;
	rdfs:label "RFC 3066"@en ;
	rdfs:isDefinedBy <http://purl.org/dc/terms/> ;
	dcterms:description "RFC 3066 has been obsoleted by RFC 4646."@en ;
	rdfs:comment "The set of tags constructed according to RFC 3066 for the identification of languages."@en ;
	dcterms:modified "2008-01-14"^^xsd:date ;
	rdfs:seeAlso <http://www.ietf.org/rfc/rfc3066.txt> ;
	dcterms:hasVersion <http://dublincore.org/usage/terms/history/#RFC3066-002> .
# 

dcterms:RFC4646 dcterms:description "RFC 4646 obsoletes RFC 3066."@en ;
	dcterms:issued "2008-01-14"^^xsd:date ;
	dcterms:hasVersion <http://dublincore.org/usage/terms/history/#RFC4646-001> ;
	rdfs:seeAlso <http://www.ietf.org/rfc/rfc4646.txt> ;
	rdfs:isDefinedBy <http://purl.org/dc/terms/> ;
	rdfs:label "RFC 4646"@en ;
	rdfs:comment "The set of tags constructed according to RFC 4646 for the identification of languages."@en .
# 

dcterms:RFC5646 dcterms:issued "2010-10-11"^^xsd:date ;
	rdfs:seeAlso <http://www.ietf.org/rfc/rfc5646.txt> ;
	dcterms:hasVersion <http://dublincore.org/usage/terms/history/#RFC5646-001> ;
	rdfs:comment "The set of tags constructed according to RFC 5646 for the identification of languages."@en ;
	rdfs:label "RFC 5646"@en ;
	dcterms:description "RFC 5646 obsoletes RFC 4646."@en ;
	rdfs:isDefinedBy <http://purl.org/dc/terms/> .
# 

dcterms:RightsStatement rdfs:label "Rights Statement"@en ;
	rdfs:isDefinedBy <http://purl.org/dc/terms/> ;
	rdfs:comment "A statement about the intellectual property rights (IPR) held in or over a Resource, a legal document giving official permission to do something with a resource, or a statement about access rights."@en ;
	dcterms:issued "2008-01-14"^^xsd:date ;
	dcterms:hasVersion <http://dublincore.org/usage/terms/history/#RightsStatement-001> .
# 

dcterms:SizeOrDuration rdfs:label "Size or Duration"@en ;
	dcterms:hasVersion <http://dublincore.org/usage/terms/history/#SizeOrDuration-001> ;
	dcterms:description "Examples include a number of pages, a specification of length, width, and breadth, or a period in hours, minutes, and seconds."@en ;
	rdfs:comment "A dimension or extent, or a time taken to play or execute."@en ;
	rdfs:isDefinedBy <http://purl.org/dc/terms/> ;
	dcterms:issued "2008-01-14"^^xsd:date .
# 

dcterms:Standard rdfs:comment "A basis for comparison; a reference point against which other things can be evaluated."@en ;
	rdfs:label "Standard"@en ;
	rdfs:isDefinedBy <http://purl.org/dc/terms/> ;
	dcterms:issued "2008-01-14"^^xsd:date ;
	dcterms:hasVersion <http://dublincore.org/usage/terms/history/#Standard-001> .
# 

dcterms:URI rdfs:comment "The set of identifiers constructed according to the generic syntax for Uniform Resource Identifiers as specified by the Internet Engineering Task Force."@en ;
	rdfs:isDefinedBy <http://purl.org/dc/terms/> ;
	dcterms:issued "2000-07-11"^^xsd:date ;
	rdfs:seeAlso <http://www.ietf.org/rfc/rfc3986.txt> ;
	dcterms:hasVersion <http://dublincore.org/usage/terms/history/#URI-003> ;
	rdfs:label "URI"@en ;
	dcterms:modified "2008-01-14"^^xsd:date .
# 

dcterms:W3CDTF rdfs:label "W3C-DTF"@en ;
	rdfs:comment "The set of dates and times constructed according to the W3C Date and Time Formats Specification."@en ;
	rdfs:isDefinedBy <http://purl.org/dc/terms/> ;
	dcterms:hasVersion <http://dublincore.org/usage/terms/history/#W3CDTF-003> ;
	dcterms:issued "2000-07-11"^^xsd:date ;
	rdfs:seeAlso <http://www.w3.org/TR/NOTE-datetime> ;
	dcterms:modified "2008-01-14"^^xsd:date .
# 

dcterms:abstract rdfs:label "Abstract"@en ;
	dcterms:modified "2008-01-14"^^xsd:date ;
	dcterms:hasVersion <http://dublincore.org/usage/terms/history/#abstract-003> ;
	dcterms:issued "2000-07-11"^^xsd:date ;
	rdfs:comment "A summary of the resource."@en ;
	rdfs:isDefinedBy <http://purl.org/dc/terms/> .
# 

dcterms:accessRights dcterms:description "Access Rights may include information regarding access or restrictions based on privacy, security, or other policies."@en ;
	dcterms:issued "2003-02-15"^^xsd:date ;
	rdfs:comment "Information about who can access the resource or an indication of its security status."@en ;
	rdfs:label "Access Rights"@en ;
	dcterms:modified "2008-01-14"^^xsd:date ;
	dcterms:hasVersion <http://dublincore.org/usage/terms/history/#accessRights-002> ;
	rdfs:isDefinedBy <http://purl.org/dc/terms/> .
# 

dcterms:accrualMethod rdfs:label "Accrual Method"@en ;
	dcterms:hasVersion <http://dublincore.org/usage/terms/history/#accrualMethod-003> ;
	dcterms:modified "2010-10-11"^^xsd:date ;
	rdfs:comment "The method by which items are added to a collection."@en ;
	rdfs:isDefinedBy <http://purl.org/dc/terms/> ;
	dcterms:issued "2005-06-13"^^xsd:date .
# 

dcterms:accrualPeriodicity dcterms:modified "2010-10-11"^^xsd:date ;
	dcterms:hasVersion <http://dublincore.org/usage/terms/history/#accrualPeriodicity-003> ;
	rdfs:label "Accrual Periodicity"@en ;
	rdfs:comment "The frequency with which items are added to a collection."@en ;
	rdfs:isDefinedBy <http://purl.org/dc/terms/> ;
	dcterms:issued "2005-06-13"^^xsd:date .
# 

dcterms:accrualPolicy rdfs:isDefinedBy <http://purl.org/dc/terms/> ;
	dcterms:issued "2005-06-13"^^xsd:date ;
	dcterms:modified "2010-10-11"^^xsd:date ;
	dcterms:hasVersion <http://dublincore.org/usage/terms/history/#accrualPolicy-003> ;
	rdfs:comment "The policy governing the addition of items to a collection."@en ;
	rdfs:label "Accrual Policy"@en .
# 

dcterms:alternative rdfs:comment "An alternative name for the resource."@en ;
	rdfs:isDefinedBy <http://purl.org/dc/terms/> ;
	dcterms:hasVersion <http://dublincore.org/usage/terms/history/#alternative-003> ;
	dcterms:modified "2010-10-11"^^xsd:date ;
	dcterms:description "The distinction between titles and alternative titles is application-specific."@en ;
	dcterms:issued "2000-07-11"^^xsd:date ;
	rdfs:label "Alternative Title"@en .
# 

dcterms:audience dcterms:issued "2001-05-21"^^xsd:date ;
	rdfs:comment "A class of entity for whom the resource is intended or useful."@en ;
	dcterms:hasVersion <http://dublincore.org/usage/terms/history/#audience-003> ;
	rdfs:label "Audience"@en ;
	rdfs:isDefinedBy <http://purl.org/dc/terms/> ;
	dcterms:modified "2008-01-14"^^xsd:date .
# 

dcterms:available rdfs:isDefinedBy <http://purl.org/dc/terms/> ;
	rdfs:comment "Date (often a range) that the resource became or will become available."@en ;
	rdfs:label "Date Available"@en ;
	dcterms:hasVersion <http://dublincore.org/usage/terms/history/#available-003> ;
	dcterms:modified "2008-01-14"^^xsd:date ;
	dcterms:issued "2000-07-11"^^xsd:date .
# 

dcterms:bibliographicCitation dcterms:modified "2008-01-14"^^xsd:date ;
	dcterms:description "Recommended practice is to include sufficient bibliographic detail to identify the resource as unambiguously as possible."@en ;
	rdfs:label "Bibliographic Citation"@en ;
	dcterms:hasVersion <http://dublincore.org/usage/terms/history/#bibliographicCitation-002> ;
	rdfs:comment "A bibliographic reference for the resource."@en ;
	rdfs:isDefinedBy <http://purl.org/dc/terms/> ;
	rdfs:label "cita bibliográfica"@es ;
	rdfs:comment "Nota, Cómo debe ser citado el dataset, por ejemplo: Marta-Costa, A., Torres-Manso, F., Pinto, R., Tibério, L.; Carneiro, I. (2016). Stakeholders’ perception of forest management: a Portuguese mountain case study. Forest Systems, Volume 25, Issue 1, e052, 13 pages. http://dx.doi.org/10.5424/fs/2016251-08122”"@es ;
	dcterms:issued "2003-02-15"^^xsd:date .
# 

dcterms:conformsTo rdfs:isDefinedBy <http://purl.org/dc/terms/> ;
	rdfs:label "Conforms To"@en ;
	rdfs:comment "An established standard to which the described resource conforms."@en ;
	dcterms:modified "2008-01-14"^^xsd:date ;
	dcterms:hasVersion <http://dublincore.org/usage/terms/history/#conformsTo-003> ;
	dcterms:issued "2001-05-21"^^xsd:date .
# 

dcterms:contributor rdfs:comment "An entity responsible for making contributions to the resource."@en ;
	dcterms:modified "2010-10-11"^^xsd:date ;
	rdfs:isDefinedBy <http://purl.org/dc/terms/> ;
	dcterms:description "Examples of a Contributor include a person, an organization, or a service."@en ;
	rdfs:comment "Colaborador en la elaboración del recurso. Esta relación puede especializarse utilizando alguna de las subpropiedades definidas de acuerdo a las necesidades de los dataset de INIA."@es ;
	dcterms:issued "2008-01-14"^^xsd:date ;
	dcterms:hasVersion <http://dublincore.org/usage/terms/history/#contributorT-001> ;
	rdfs:label "Contributor"@en , "colaborador"@es .
# 

dcterms:coverage rdfs:isDefinedBy <http://purl.org/dc/terms/> ;
	dcterms:hasVersion <http://dublincore.org/usage/terms/history/#coverageT-001> ;
	dcterms:description "Spatial topic and spatial applicability may be a named place or a location specified by its geographic coordinates. Temporal topic may be a named period, date, or date range. A jurisdiction may be a named administrative entity or a geographic place to which the resource applies. Recommended best practice is to use a controlled vocabulary such as the Thesaurus of Geographic Names [TGN]. Where appropriate, named places or time periods can be used in preference to numeric identifiers such as sets of coordinates or date ranges."@en ;
	rdfs:label "Coverage"@en ;
	dcterms:issued "2008-01-14"^^xsd:date ;
	rdfs:comment "The spatial or temporal topic of the resource, the spatial applicability of the resource, or the jurisdiction under which the resource is relevant."@en ;
	dcterms:modified "2008-01-14"^^xsd:date .
# 

dcterms:created rdfs:isDefinedBy <http://purl.org/dc/terms/> ;
	rdfs:comment "Date of creation of the resource."@en ;
	dcterms:hasVersion <http://dublincore.org/usage/terms/history/#created-003> ;
	dcterms:modified "2008-01-14"^^xsd:date ;
	rdfs:label "Date Created"@en ;
	dcterms:issued "2000-07-11"^^xsd:date .
# 

dcterms:creator rdfs:comment "An entity primarily responsible for making the resource."@en ;
	rdfs:label "autor"@es ;
	dcterms:hasVersion <http://dublincore.org/usage/terms/history/#creatorT-002> ;
	rdfs:isDefinedBy <http://purl.org/dc/terms/> ;
	dcterms:modified "2010-10-11"^^xsd:date ;
	rdfs:comment "Indica el autor o los autores del recurso."@es ;
	dcterms:issued "2008-01-14"^^xsd:date ;
	rdfs:label "Creator"@en ;
	dcterms:description "Examples of a Creator include a person, an organization, or a service."@en .
# 

dcterms:date rdfs:isDefinedBy <http://purl.org/dc/terms/> ;
	dcterms:hasVersion <http://dublincore.org/usage/terms/history/#dateT-001> ;
	rdfs:comment "A point or period of time associated with an event in the lifecycle of the resource."@en ;
	dcterms:description "Date may be used to express temporal information at any level of granularity.  Recommended best practice is to use an encoding scheme, such as the W3CDTF profile of ISO 8601 [W3CDTF]."@en ;
	rdfs:label "Date"@en ;
	dcterms:issued "2008-01-14"^^xsd:date ;
	dcterms:modified "2008-01-14"^^xsd:date .
# 

dcterms:dateAccepted dcterms:modified "2008-01-14"^^xsd:date ;
	dcterms:hasVersion <http://dublincore.org/usage/terms/history/#dateAccepted-002> ;
	dcterms:issued "2002-07-13"^^xsd:date ;
	dcterms:description "Examples of resources to which a Date Accepted may be relevant are a thesis (accepted by a university department) or an article (accepted by a journal)."@en ;
	rdfs:label "Date Accepted"@en ;
	rdfs:comment "Date of acceptance of the resource."@en ;
	rdfs:isDefinedBy <http://purl.org/dc/terms/> .
# 

dcterms:dateCopyrighted rdfs:isDefinedBy <http://purl.org/dc/terms/> ;
	rdfs:label "Date Copyrighted"@en ;
	rdfs:comment "Date of copyright."@en ;
	dcterms:modified "2008-01-14"^^xsd:date ;
	dcterms:hasVersion <http://dublincore.org/usage/terms/history/#dateCopyrighted-002> ;
	dcterms:issued "2002-07-13"^^xsd:date .
# 

dcterms:dateSubmitted dcterms:modified "2008-01-14"^^xsd:date ;
	rdfs:comment "Date of submission of the resource."@en ;
	dcterms:description "Examples of resources to which a Date Submitted may be relevant are a thesis (submitted to a university department) or an article (submitted to a journal)."@en ;
	dcterms:issued "2002-07-13"^^xsd:date ;
	rdfs:label "Date Submitted"@en ;
	dcterms:hasVersion <http://dublincore.org/usage/terms/history/#dateSubmitted-002> ;
	rdfs:isDefinedBy <http://purl.org/dc/terms/> .
# 

dcterms:description dcterms:modified "2008-01-14"^^xsd:date ;
	rdfs:label "Description"@en ;
	rdfs:comment "Resumen, descripción, información de interés sobre el dataset."@es ;
	rdfs:label "descripción"@es ;
	rdfs:isDefinedBy <http://purl.org/dc/terms/> ;
	rdfs:comment "An account of the resource."@en ;
	dcterms:issued "2008-01-14"^^xsd:date ;
	dcterms:hasVersion <http://dublincore.org/usage/terms/history/#descriptionT-001> ;
	dcterms:description "Description may include but is not limited to: an abstract, a table of contents, a graphical representation, or a free-text account of the resource."@en .
# 

dcterms:educationLevel dcterms:modified "2008-01-14"^^xsd:date ;
	rdfs:isDefinedBy <http://purl.org/dc/terms/> ;
	dcterms:issued "2002-07-13"^^xsd:date ;
	rdfs:label "Audience Education Level"@en ;
	rdfs:comment "A class of entity, defined in terms of progression through an educational or training context, for which the described resource is intended."@en ;
	dcterms:hasVersion <http://dublincore.org/usage/terms/history/#educationLevel-002> .
# 

dcterms:extent dcterms:modified "2008-01-14"^^xsd:date ;
	dcterms:issued "2000-07-11"^^xsd:date ;
	rdfs:isDefinedBy <http://purl.org/dc/terms/> ;
	rdfs:comment "The size or duration of the resource."@en ;
	rdfs:label "Extent"@en ;
	dcterms:hasVersion <http://dublincore.org/usage/terms/history/#extent-003> .
# 

dcterms:format dcterms:issued "2008-01-14"^^xsd:date ;
	dcterms:hasVersion <http://dublincore.org/usage/terms/history/#formatT-001> ;
	dcterms:modified "2008-01-14"^^xsd:date ;
	rdfs:comment "The file format, physical medium, or dimensions of the resource."@en ;
	dcterms:description "Examples of dimensions include size and duration. Recommended best practice is to use a controlled vocabulary such as the list of Internet Media Types [MIME]."@en ;
	rdfs:isDefinedBy <http://purl.org/dc/terms/> ;
	rdfs:label "Format"@en .
# 

dcterms:hasFormat rdfs:isDefinedBy <http://purl.org/dc/terms/> ;
	<http://www.w3.org/2004/02/skos/core#note> "This term is intended to be used with non-literal values as defined in the DCMI Abstract Model (http://dublincore.org/documents/abstract-model/).  As of December 2007, the DCMI Usage Board is seeking a way to express this intention with a formal range declaration."@en ;
	dcterms:hasVersion <http://dublincore.org/usage/terms/history/#hasFormat-003> ;
	dcterms:modified "2008-01-14"^^xsd:date ;
	rdfs:label "Has Format"@en ;
	rdfs:comment "A related resource that is substantially the same as the pre-existing described resource, but in another format."@en ;
	dcterms:issued "2000-07-11"^^xsd:date .
# 

dcterms:hasPart rdfs:isDefinedBy <http://purl.org/dc/terms/> ;
	<http://www.w3.org/2004/02/skos/core#note> "This term is intended to be used with non-literal values as defined in the DCMI Abstract Model (http://dublincore.org/documents/abstract-model/).  As of December 2007, the DCMI Usage Board is seeking a way to express this intention with a formal range declaration."@en ;
	dcterms:issued "2000-07-11"^^xsd:date ;
	rdfs:label "Has Part"@en ;
	dcterms:modified "2008-01-14"^^xsd:date ;
	rdfs:comment "A related resource that is included either physically or logically in the described resource."@en ;
	dcterms:hasVersion <http://dublincore.org/usage/terms/history/#hasPart-003> .
# 

dcterms:hasVersion dcterms:hasVersion <http://dublincore.org/usage/terms/history/#hasVersion-003> ;
	rdfs:isDefinedBy <http://purl.org/dc/terms/> ;
	rdfs:comment "A related resource that is a version, edition, or adaptation of the described resource."@en ;
	<http://www.w3.org/2004/02/skos/core#note> "This term is intended to be used with non-literal values as defined in the DCMI Abstract Model (http://dublincore.org/documents/abstract-model/).  As of December 2007, the DCMI Usage Board is seeking a way to express this intention with a formal range declaration."@en ;
	rdfs:label "Has Version"@en ;
	dcterms:issued "2000-07-11"^^xsd:date ;
	dcterms:modified "2008-01-14"^^xsd:date .
# 

dcterms:identifier dcterms:hasVersion <http://dublincore.org/usage/terms/history/#identifierT-001> ;
	rdfs:isDefinedBy <http://purl.org/dc/terms/> ;
	dcterms:description "Recommended best practice is to identify the resource by means of a string conforming to a formal identification system. "@en ;
	dcterms:modified "2008-01-14"^^xsd:date ;
	rdfs:comment "An unambiguous reference to the resource within a given context."@en ;
	rdfs:label "Identifier"@en ;
	dcterms:issued "2008-01-14"^^xsd:date .
# 

dcterms:instructionalMethod dcterms:issued "2005-06-13"^^xsd:date ;
	dcterms:description "Instructional Method will typically include ways of presenting instructional materials or conducting instructional activities, patterns of learner-to-learner and learner-to-instructor interactions, and mechanisms by which group and individual levels of learning are measured.  Instructional methods include all aspects of the instruction and learning processes from planning and implementation through evaluation and feedback."@en ;
	rdfs:label "Instructional Method"@en ;
	dcterms:modified "2008-01-14"^^xsd:date ;
	rdfs:comment "A process, used to engender knowledge, attitudes and skills, that the described resource is designed to support."@en ;
	dcterms:hasVersion <http://dublincore.org/usage/terms/history/#instructionalMethod-002> ;
	rdfs:isDefinedBy <http://purl.org/dc/terms/> .
# 

dcterms:isFormatOf dcterms:hasVersion <http://dublincore.org/usage/terms/history/#isFormatOf-003> ;
	dcterms:modified "2008-01-14"^^xsd:date ;
	rdfs:comment "A related resource that is substantially the same as the described resource, but in another format."@en ;
	dcterms:issued "2000-07-11"^^xsd:date ;
	<http://www.w3.org/2004/02/skos/core#note> "This term is intended to be used with non-literal values as defined in the DCMI Abstract Model (http://dublincore.org/documents/abstract-model/).  As of December 2007, the DCMI Usage Board is seeking a way to express this intention with a formal range declaration."@en ;
	rdfs:label "Is Format Of"@en ;
	rdfs:isDefinedBy <http://purl.org/dc/terms/> .
# 

dcterms:isPartOf dcterms:modified "2008-01-14"^^xsd:date ;
	rdfs:label "Is Part Of"@en ;
	dcterms:hasVersion <http://dublincore.org/usage/terms/history/#isPartOf-003> ;
	dcterms:issued "2000-07-11"^^xsd:date ;
	<http://www.w3.org/2004/02/skos/core#note> "This term is intended to be used with non-literal values as defined in the DCMI Abstract Model (http://dublincore.org/documents/abstract-model/).  As of December 2007, the DCMI Usage Board is seeking a way to express this intention with a formal range declaration."@en ;
	rdfs:isDefinedBy <http://purl.org/dc/terms/> ;
	rdfs:comment "A related resource in which the described resource is physically or logically included."@en .
# 

dcterms:isReferencedBy rdfs:label "Is Referenced By"@en ;
	rdfs:comment "A related resource that references, cites, or otherwise points to the described resource."@en ;
	dcterms:modified "2008-01-14"^^xsd:date ;
	<http://www.w3.org/2004/02/skos/core#note> "This term is intended to be used with non-literal values as defined in the DCMI Abstract Model (http://dublincore.org/documents/abstract-model/).  As of December 2007, the DCMI Usage Board is seeking a way to express this intention with a formal range declaration."@en ;
	rdfs:isDefinedBy <http://purl.org/dc/terms/> ;
	dcterms:issued "2000-07-11"^^xsd:date ;
	dcterms:hasVersion <http://dublincore.org/usage/terms/history/#isReferencedBy-003> .
# 

dcterms:isReplacedBy rdfs:isDefinedBy <http://purl.org/dc/terms/> ;
	rdfs:label "Is Replaced By"@en ;
	dcterms:modified "2008-01-14"^^xsd:date ;
	rdfs:comment "A related resource that supplants, displaces, or supersedes the described resource."@en ;
	dcterms:issued "2000-07-11"^^xsd:date ;
	<http://www.w3.org/2004/02/skos/core#note> "This term is intended to be used with non-literal values as defined in the DCMI Abstract Model (http://dublincore.org/documents/abstract-model/).  As of December 2007, the DCMI Usage Board is seeking a way to express this intention with a formal range declaration."@en ;
	dcterms:hasVersion <http://dublincore.org/usage/terms/history/#isReplacedBy-003> .
# 

dcterms:isRequiredBy rdfs:isDefinedBy <http://purl.org/dc/terms/> ;
	<http://www.w3.org/2004/02/skos/core#note> "This term is intended to be used with non-literal values as defined in the DCMI Abstract Model (http://dublincore.org/documents/abstract-model/).  As of December 2007, the DCMI Usage Board is seeking a way to express this intention with a formal range declaration."@en ;
	dcterms:issued "2000-07-11"^^xsd:date ;
	rdfs:label "Is Required By"@en ;
	dcterms:hasVersion <http://dublincore.org/usage/terms/history/#isRequiredBy-003> ;
	dcterms:modified "2008-01-14"^^xsd:date ;
	rdfs:comment "A related resource that requires the described resource to support its function, delivery, or coherence."@en .
# 

dcterms:isVersionOf rdfs:label "Is Version Of"@en ;
	rdfs:comment "A related resource of which the described resource is a version, edition, or adaptation."@en ;
	rdfs:isDefinedBy <http://purl.org/dc/terms/> ;
	dcterms:issued "2000-07-11"^^xsd:date ;
	<http://www.w3.org/2004/02/skos/core#note> "This term is intended to be used with non-literal values as defined in the DCMI Abstract Model (http://dublincore.org/documents/abstract-model/).  As of December 2007, the DCMI Usage Board is seeking a way to express this intention with a formal range declaration."@en ;
	dcterms:hasVersion <http://dublincore.org/usage/terms/history/#isVersionOf-003> ;
	dcterms:modified "2008-01-14"^^xsd:date ;
	dcterms:description "Changes in version imply substantive changes in content rather than differences in format."@en .
# 

dcterms:issued rdfs:label "fecha de publicación"@es ;
	dcterms:modified "2008-01-14"^^xsd:date ;
	rdfs:comment "Date of formal issuance (e.g., publication) of the resource."@en , "Fecha en la que se introduce por primera vez el dataset a REDIA."@es ;
	rdfs:isDefinedBy <http://purl.org/dc/terms/> ;
	dcterms:hasVersion <http://dublincore.org/usage/terms/history/#issued-003> ;
	dcterms:issued "2000-07-11"^^xsd:date ;
	rdfs:label "Date Issued"@en .
# 

dcterms:language rdfs:label "Language"@en ;
	dcterms:issued "2008-01-14"^^xsd:date ;
	dcterms:hasVersion <http://dublincore.org/usage/terms/history/#languageT-001> ;
	dcterms:modified "2008-01-14"^^xsd:date ;
	rdfs:label "idioma"@es ;
	dcterms:description "Recommended best practice is to use a controlled vocabulary such as RFC 4646 [RFC4646]."@en ;
	rdfs:comment "Relación que indica el idioma del dataset. En el objeto se esperan instancias de la clase lvon:language"@es ;
	rdfs:isDefinedBy <http://purl.org/dc/terms/> ;
	rdfs:comment "A language of the resource."@en .
# 

dcterms:license rdfs:comment "licencia"@es ;
	dcterms:issued "2004-06-14"^^xsd:date ;
	rdfs:label "License"@en ;
	rdfs:comment "A legal document giving official permission to do something with the resource."@en ;
	dcterms:hasVersion <http://dublincore.org/usage/terms/history/#license-002> ;
	rdfs:comment "Licencia que especifica los permisos para hacer algo con el recurso."@es ;
	dcterms:modified "2008-01-14"^^xsd:date ;
	rdfs:isDefinedBy <http://purl.org/dc/terms/> .
# 

dcterms:mediator dcterms:description "In an educational context, a mediator might be a parent, teacher, teaching assistant, or care-giver."@en ;
	dcterms:modified "2008-01-14"^^xsd:date ;
	rdfs:comment "An entity that mediates access to the resource and for whom the resource is intended or useful."@en ;
	dcterms:hasVersion <http://dublincore.org/usage/terms/history/#mediator-003> ;
	rdfs:isDefinedBy <http://purl.org/dc/terms/> ;
	rdfs:label "Mediator"@en ;
	dcterms:issued "2001-05-21"^^xsd:date .
# 

dcterms:medium rdfs:isDefinedBy <http://purl.org/dc/terms/> ;
	rdfs:label "Medium"@en ;
	rdfs:comment "The material or physical carrier of the resource."@en ;
	dcterms:issued "2000-07-11"^^xsd:date ;
	dcterms:modified "2008-01-14"^^xsd:date ;
	dcterms:hasVersion <http://dublincore.org/usage/terms/history/#medium-003> .
# 

dcterms:modified rdfs:isDefinedBy <http://purl.org/dc/terms/> ;
	rdfs:label "Date Modified"@en ;
	dcterms:hasVersion <http://dublincore.org/usage/terms/history/#modified-003> ;
	dcterms:modified "2008-01-14"^^xsd:date ;
	rdfs:comment "Date on which the resource was changed."@en ;
	dcterms:issued "2000-07-11"^^xsd:date .
# 

dcterms:provenance rdfs:comment "A statement of any changes in ownership and custody of the resource since its creation that are significant for its authenticity, integrity, and interpretation."@en ;
	dcterms:modified "2008-01-14"^^xsd:date ;
	dcterms:issued "2004-09-20"^^xsd:date ;
	rdfs:isDefinedBy <http://purl.org/dc/terms/> ;
	dcterms:description "The statement may include a description of any changes successive custodians made to the resource."@en ;
	dcterms:hasVersion <http://dublincore.org/usage/terms/history/#provenance-002> ;
	rdfs:label "Provenance"@en .
# 

dcterms:publisher dcterms:modified "2010-10-11"^^xsd:date ;
	dcterms:issued "2008-01-14"^^xsd:date ;
	rdfs:label "Publisher"@en ;
	dcterms:hasVersion <http://dublincore.org/usage/terms/history/#publisherT-001> ;
	dcterms:description "Examples of a Publisher include a person, an organization, or a service."@en ;
	rdfs:isDefinedBy <http://purl.org/dc/terms/> ;
	rdfs:comment "An entity responsible for making the resource available."@en .
# 

dcterms:references rdfs:comment "A related resource that is referenced, cited, or otherwise pointed to by the described resource."@en ;
	rdfs:label "References"@en ;
	dcterms:modified "2008-01-14"^^xsd:date ;
	dcterms:issued "2000-07-11"^^xsd:date ;
	dcterms:hasVersion <http://dublincore.org/usage/terms/history/#references-003> ;
	rdfs:isDefinedBy <http://purl.org/dc/terms/> ;
	<http://www.w3.org/2004/02/skos/core#note> "This term is intended to be used with non-literal values as defined in the DCMI Abstract Model (http://dublincore.org/documents/abstract-model/).  As of December 2007, the DCMI Usage Board is seeking a way to express this intention with a formal range declaration."@en .
# 

dcterms:relation dcterms:issued "2008-01-14"^^xsd:date ;
	<http://www.w3.org/2004/02/skos/core#note> "This term is intended to be used with non-literal values as defined in the DCMI Abstract Model (http://dublincore.org/documents/abstract-model/).  As of December 2007, the DCMI Usage Board is seeking a way to express this intention with a formal range declaration."@en ;
	rdfs:isDefinedBy <http://purl.org/dc/terms/> ;
	dcterms:hasVersion <http://dublincore.org/usage/terms/history/#relationT-001> ;
	rdfs:label "Relation"@en ;
	dcterms:description "Recommended best practice is to identify the related resource by means of a string conforming to a formal identification system. "@en ;
	rdfs:comment "A related resource."@en ;
	dcterms:modified "2008-01-14"^^xsd:date .
# 

dcterms:replaces <http://www.w3.org/2004/02/skos/core#note> "This term is intended to be used with non-literal values as defined in the DCMI Abstract Model (http://dublincore.org/documents/abstract-model/).  As of December 2007, the DCMI Usage Board is seeking a way to express this intention with a formal range declaration."@en ;
	dcterms:issued "2000-07-11"^^xsd:date ;
	dcterms:modified "2008-01-14"^^xsd:date ;
	rdfs:label "Replaces"@en ;
	dcterms:hasVersion <http://dublincore.org/usage/terms/history/#replaces-003> ;
	rdfs:comment "A related resource that is supplanted, displaced, or superseded by the described resource."@en ;
	rdfs:isDefinedBy <http://purl.org/dc/terms/> .
# 

dcterms:requires dcterms:hasVersion <http://dublincore.org/usage/terms/history/#requires-003> ;
	dcterms:modified "2008-01-14"^^xsd:date ;
	rdfs:label "Requires"@en ;
	rdfs:comment "A related resource that is required by the described resource to support its function, delivery, or coherence."@en ;
	rdfs:isDefinedBy <http://purl.org/dc/terms/> ;
	dcterms:issued "2000-07-11"^^xsd:date ;
	<http://www.w3.org/2004/02/skos/core#note> "This term is intended to be used with non-literal values as defined in the DCMI Abstract Model (http://dublincore.org/documents/abstract-model/).  As of December 2007, the DCMI Usage Board is seeking a way to express this intention with a formal range declaration."@en .
# 

dcterms:rights rdfs:isDefinedBy <http://purl.org/dc/terms/> ;
	dcterms:issued "2008-01-14"^^xsd:date ;
	rdfs:label "Rights"@en ;
	rdfs:comment "Information about rights held in and over the resource."@en ;
	dcterms:modified "2008-01-14"^^xsd:date ;
	rdfs:comment "Derechos de utilización del recurso."@es ;
	rdfs:label "derechos de utilización"@es ;
	dcterms:hasVersion <http://dublincore.org/usage/terms/history/#rightsT-001> ;
	dcterms:description "Typically, rights information includes a statement about various property rights associated with the resource, including intellectual property rights."@en .
# 

dcterms:rightsHolder dcterms:hasVersion <http://dublincore.org/usage/terms/history/#rightsHolder-002> ;
	rdfs:isDefinedBy <http://purl.org/dc/terms/> ;
	dcterms:modified "2008-01-14"^^xsd:date ;
	rdfs:comment "A person or organization owning or managing rights over the resource."@en ;
	dcterms:issued "2004-06-14"^^xsd:date ;
	rdfs:label "Rights Holder"@en .
# 

dcterms:source rdfs:label "Source"@en ;
	<http://www.w3.org/2004/02/skos/core#note> "This term is intended to be used with non-literal values as defined in the DCMI Abstract Model (http://dublincore.org/documents/abstract-model/).  As of December 2007, the DCMI Usage Board is seeking a way to express this intention with a formal range declaration."@en ;
	dcterms:issued "2008-01-14"^^xsd:date ;
	rdfs:isDefinedBy <http://purl.org/dc/terms/> ;
	dcterms:modified "2008-01-14"^^xsd:date ;
	dcterms:hasVersion <http://dublincore.org/usage/terms/history/#sourceT-001> ;
	rdfs:comment "A related resource from which the described resource is derived."@en ;
	dcterms:description "The described resource may be derived from the related resource in whole or in part. Recommended best practice is to identify the related resource by means of a string conforming to a formal identification system."@en .
# 

dcterms:spatial dcterms:issued "2000-07-11"^^xsd:date ;
	rdfs:label "Spatial Coverage"@en ;
	rdfs:comment "Alternativa a inia:spatialScope para indicar el ámbito geográfivo. Se puede expresar mediante la localización de un punto (latitud_N y longitud_W ), o por un rectángulo (latitud N, longitud E, latitud S y longitud W ) mediante la clase ext:GeographicBoundingBox"@es ;
	rdfs:isDefinedBy <http://purl.org/dc/terms/> ;
	rdfs:comment "Spatial characteristics of the resource."@en ;
	dcterms:modified "2008-01-14"^^xsd:date ;
	dcterms:hasVersion <http://dublincore.org/usage/terms/history/#spatial-003> .
# 

dcterms:subject dcterms:modified "2012-06-14"^^xsd:date ;
	dcterms:hasVersion <http://dublincore.org/usage/terms/history/#subjectT-002> ;
	<http://www.w3.org/2004/02/skos/core#note> "This term is intended to be used with non-literal values as defined in the DCMI Abstract Model (http://dublincore.org/documents/abstract-model/).  As of December 2007, the DCMI Usage Board is seeking a way to express this intention with a formal range declaration."@en ;
	dcterms:issued "2008-01-14"^^xsd:date ;
	rdfs:label "Subject"@en ;
	rdfs:comment "The topic of the resource."@en ;
	dcterms:description "Typically, the subject will be represented using keywords, key phrases, or classification codes. Recommended best practice is to use a controlled vocabulary."@en ;
	rdfs:isDefinedBy <http://purl.org/dc/terms/> .
# 

dcterms:tableOfContents rdfs:comment "A list of subunits of the resource."@en ;
	dcterms:issued "2000-07-11"^^xsd:date ;
	rdfs:isDefinedBy <http://purl.org/dc/terms/> ;
	rdfs:label "Table Of Contents"@en ;
	dcterms:modified "2008-01-14"^^xsd:date ;
	dcterms:hasVersion <http://dublincore.org/usage/terms/history/#tableOfContents-003> .
# 

dcterms:temporal dcterms:modified "2008-01-14"^^xsd:date ;
	rdfs:label "ambito temporal"@es ;
	dcterms:issued "2000-07-11"^^xsd:date ;
	rdfs:comment "Se podría utilizar esta propiedad como alternataiva a inia:startingDate e inia:finalDate cuando el objeto de la relación se represente con una instancia de time:Interval."@es ;
	rdfs:label "Temporal Coverage"@en ;
	dcterms:hasVersion <http://dublincore.org/usage/terms/history/#temporal-003> ;
	rdfs:comment "Temporal characteristics of the resource."@en ;
	rdfs:isDefinedBy <http://purl.org/dc/terms/> .
# 

dcterms:title rdfs:label "Title"@en ;
	rdfs:comment "A name given to the resource."@en ;
	rdfs:label "título"@es ;
	dcterms:issued "2008-01-14"^^xsd:date ;
	rdfs:label "Título del dataset. Al menos debe tener uno."@es ;
	dcterms:hasVersion <http://dublincore.org/usage/terms/history/#titleT-002> ;
	rdfs:isDefinedBy <http://purl.org/dc/terms/> ;
	dcterms:modified "2010-10-11"^^xsd:date .
# 

dcterms:type rdfs:isDefinedBy <http://purl.org/dc/terms/> ;
	dcterms:description "Recommended best practice is to use a controlled vocabulary such as the DCMI Type Vocabulary [DCMITYPE]. To describe the file format, physical medium, or dimensions of the resource, use the Format element."@en ;
	rdfs:comment "The nature or genre of the resource."@en ;
	dcterms:modified "2008-01-14"^^xsd:date ;
	rdfs:label "Type"@en ;
	dcterms:hasVersion <http://dublincore.org/usage/terms/history/#typeT-001> ;
	dcterms:issued "2008-01-14"^^xsd:date .
# 

dcterms:valid rdfs:comment "Date (often a range) of validity of a resource."@en ;
	dcterms:modified "2008-01-14"^^xsd:date ;
	dcterms:issued "2000-07-11"^^xsd:date ;
	rdfs:label "Date Valid"@en ;
	dcterms:hasVersion <http://dublincore.org/usage/terms/history/#valid-003> ;
	rdfs:isDefinedBy <http://purl.org/dc/terms/> .
# 

<http://purl.org/spar/datacite/usesIdentifierScheme> rdfs:label "utiliza esquema de identificadores"@es ;
	rdfs:comment "Una propiedad que permite la especificación del esquema de identificador utilizado para proporcionar el identificador de una entidad - ya sea un financiador, una persona o un recurso - definido como un individuo de la clase datacite:IdentifierScheme."@es .
# 

foaf:Agent rdfs:comment "Un agente (por ejemplo, persona, grupo, software o artefacto físico)."@es ;
	rdfs:label "Agente"@es .
# 
# Generated by the OWL API (version 4.2.6.20160910-2108) https://github.com/owlcs/owlapi
